.

LC.v
@@ -1703,920 +1703,2691 @@ Proof with eauto with *.
 Qed.
 
 End DomainTheory.
+Require Import Coq.Arith.PeanoNat.
+Require Import Coq.Bool.Bool.
+Require Import Coq.Classes.RelationClasses.
+Require Import Coq.Logic.Classical.
+Require Import Coq.Logic.FunctionalExtensionality.
+Require Import Coq.Logic.PropExtensionality.
+Require Import Coq.Lists.List.
+Require Import Coq.micromega.Lia.
+Require Import Coq.Program.Basics.
 
-Module UntypedLamdbdaCalculus.
+Global Create HintDb my_hints.
+
+Module MyUtilities.
+
+  Definition case_eq {A : Type} : forall x : A, forall y : A, forall phi : forall x0 : A, x0 = y -> Type, phi y eq_refl -> forall H : x = y, phi x H :=
+    fun x : A =>
+    fun y : A =>
+    fun phi : forall x0 : A, x0 = y -> Type =>
+    fun phi_y : phi y eq_refl =>
+    fun H : eq x y =>
+    match H as H0 in eq _ y0 return forall phi0 : forall x0 : A, x0 = y0 -> Type, phi0 y0 eq_refl -> phi0 x H0 with
+    | eq_refl =>
+      fun phi0 : forall x0 : A, x0 = x -> Type =>
+      fun phi_y0 : phi0 x eq_refl =>
+      phi_y0
+    end phi phi_y
+  .
+
+  Lemma div_mod_uniqueness :
+    forall a : nat,
+    forall b : nat,
+    forall q : nat,
+    forall r : nat,
+    a = b * q + r ->
+    r < b ->
+    a / b = q /\ a mod b = r.
+  Proof with try (lia || now (firstorder; eauto)).
+    assert (H : forall x : nat, forall y : nat, x > y <-> (exists z : nat, x = S (y + z))).
+    { intros x y; constructor.
+      - intros H.
+        induction H...
+        destruct IHle as [z H0].
+        exists (S z)...
+      - intros H.
+        destruct H as [z H]...
+    }
+    intros a b q r H1 H2.
+    assert (H0 : a = b * (a / b) + (a mod b)) by now apply (Nat.div_mod a b); lia.
+    assert (H3 : 0 <= a mod b < b) by now apply (Nat.mod_bound_pos a b); lia.
+    assert (H4 : ~ q > a / b).
+    { intros H4.
+      enough (H5 : exists z : nat, q = S (a / b + z))...
+      destruct H5 as [z H5].
+      enough (b * q + r >= b * S (a / b) + r)...
+    }
+    assert (H5 : ~ q < a / b).
+    { intros H5.
+      enough (H6 : exists z : nat, a / b = S (q + z))...
+      destruct H6 as [z H6].
+      enough (b * q + a mod b >= b * S (a / b) + a mod b)...
+    }
+    enough (q = a / b)...
+  Qed.
+
+  Definition first_nat : (nat -> bool) -> nat -> nat :=
+    fun p : nat -> bool =>
+    fix first_nat_fix (n : nat) {struct n} : nat :=
+    match n with
+    | 0 => 0
+    | S n' => if p (first_nat_fix n') then first_nat_fix n' else n
+    end
+  .
+
+  Theorem well_ordering_principle : 
+    forall p : nat -> bool,
+    forall n : nat,
+    p n = true ->
+    let m : nat := first_nat p n in
+    p m = true /\ (forall i : nat, p i = true -> i >= m).
+  Proof with eauto. (* This proof has been improved by JunYoung Clare Jang. *)
+    intros p n H3 m.
+    assert (forall x : nat, p x = true -> p (first_nat p x) = true).
+    { induction x...
+      simpl.
+      destruct (p (first_nat p x)) eqn:H0...
+    }
+    split...
+    intros i H4.
+    enough (forall x : nat, first_nat p x <= x).
+    enough (forall x : nat, p (first_nat p x) = true -> (forall y : nat, x < y -> first_nat p x = first_nat p y)).
+    enough (forall x : nat, forall y : nat, p y = true -> first_nat p x <= y)...
+    - intros x y H2.
+      destruct (Compare_dec.le_lt_dec x y).
+      + eapply Nat.le_trans...
+      + replace (first_nat p x) with (first_nat p y)...
+    - intros x H1 y H2.
+      induction H2; simpl.
+      + rewrite H1...
+      + rewrite <- IHle, H1...
+    - induction x...
+      simpl.
+      destruct (p (first_nat p x)) eqn: H0...
+  Qed.
+
+  Fixpoint sum_from_0_to (n : nat) {struct n} : nat :=
+    match n with
+    | 0 => 0
+    | S n' => n + sum_from_0_to n'
+    end
+  .
+
+  Proposition sum_from_0_to_is :
+    forall n : nat,
+    2 * sum_from_0_to n = n * (S n).
+  Proof with lia.
+    induction n; simpl in *...
+  Qed.
+
+  Fixpoint cantor_pairing (n : nat) {struct n} : nat * nat :=
+    match n with
+    | 0 => (0, 0)
+    | S n' =>
+      match cantor_pairing n' with
+      | (0, y) => (S y, 0)
+      | (S x, y) => (x, S y)
+      end
+    end
+  .
+
+  Lemma cantor_pairing_is_surjective :
+    forall x : nat,
+    forall y : nat,
+    (x, y) = cantor_pairing (sum_from_0_to (x + y) + y).
+  Proof with (lia || eauto).
+    enough (forall z : nat, forall y : nat, forall x : nat, z = x + y -> (x, y) = cantor_pairing (sum_from_0_to z + y))...
+    induction z.
+    - intros y x H.
+      assert (H0 : x = 0)...
+      assert (H1 : y = 0)...
+      subst...
+    - induction y.
+      + intros x H.
+        assert (H0 : x = S z)...
+        subst.
+        simpl.
+        destruct (cantor_pairing (z + sum_from_0_to z + 0)) eqn: H0.
+        assert (H1 : (0, z) = cantor_pairing (sum_from_0_to z + z))...
+        rewrite Nat.add_0_r, Nat.add_comm in H0.
+        rewrite H0 in H1.
+        inversion H1; subst...
+      + intros x H.
+        enough (H0 : (S x, y) = cantor_pairing (sum_from_0_to (S z) + y)).
+        { assert (H1 : z + sum_from_0_to z + S y = sum_from_0_to (S z) + y) by now simpl...
+          simpl.
+          rewrite H1, <- H0...
+        }
+        apply (IHy (S x))...
+  Qed.
+
+  Lemma cantor_pairing_is_injective :
+    forall n : nat,
+    forall x : nat,
+    forall y : nat,
+    cantor_pairing n = (x, y) ->
+    n = sum_from_0_to (x + y) + y.
+  Proof with (lia || eauto).
+    induction n; simpl.
+    - intros x y H.
+      inversion H; subst...
+    - intros x y H.
+      destruct (cantor_pairing n) as [x' y'] eqn: H0.
+      destruct x'; (inversion H; subst).
+      + repeat (rewrite Nat.add_0_r).
+        simpl.
+        rewrite (IHn 0 y' eq_refl), Nat.add_0_l...
+      + rewrite (IHn (S x) y' eq_refl).
+        assert (H1 : forall x' : nat, S x' + y' = x' + S y')...
+        repeat (rewrite H1)...
+  Qed.
+
+  Corollary cantor_pairing_is :
+    forall n : nat,
+    forall x : nat,
+    forall y : nat,
+    cantor_pairing n = (x, y) <-> n = sum_from_0_to (x + y) + y.
+  Proof with eauto using cantor_pairing_is_injective, cantor_pairing_is_surjective.
+    split...
+    intros H.
+    subst...
+  Qed.
+
+  Definition S_0 {A : Type} : forall n : nat, S n = 0 -> A :=
+    fun n : nat =>
+    fun H0 : S n = 0 =>
+    let H1 : 0 = S n := @eq_ind nat (S n) (fun x : nat => x = S n) eq_refl 0 H0 in
+    let H2 : False := @eq_ind nat 0 (fun x : nat => if Nat.eqb x 0 then True else False) I (S n) H1 in
+    False_rect A H2
+  .
+
+  Definition S_S : forall n1 : nat, forall n2 : nat, S n1 = S n2 -> n1 = n2 :=
+    fun n1 : nat =>
+    fun n2 : nat =>
+    fun H0 : S n1 = S n2 =>
+    @eq_ind nat (S n1) (fun x : nat => n1 = pred x) eq_refl (S n2) H0
+  .
+
+  Inductive FinSet : nat -> Set :=
+  | FZ : forall n : nat, FinSet (S n) 
+  | FS : forall n : nat, FinSet n -> FinSet (S n)
+  .
+
+  Definition FinSet_case0 {P : FinSet 0 -> Type} : forall i : FinSet 0, P i :=
+    fun i : FinSet 0 =>
+    match i as i0 in FinSet Sn return Sn = 0 -> P i with
+    | FZ n => S_0 n
+    | FS n i' => S_0 n
+    end eq_refl
+  .
+
+  Definition FinSet_caseS {n : nat} {P : FinSet (S n) -> Type} : P (FZ n) -> (forall i' : FinSet n, P (FS n i')) -> (forall i : FinSet (S n), P i) :=
+    fun PZ : P (FZ n) =>
+    fun PS : forall i' : FinSet n, P (FS n i') =>
+    fun i : FinSet (S n) =>
+    match i as i0 in FinSet Sn0 return (match Sn0 as Sn1 return FinSet Sn1 -> Type with 0 => FinSet_case0 | S n0 => fun i1 : FinSet (S n0) => forall P0 : FinSet (S n0) -> Type, P0 (FZ n0) -> (forall i' : FinSet n0, P0 (FS n0 i')) -> P0 i1 end) i0 with
+    | FZ n0 => fun P0 : FinSet (S n0) -> Type => fun PZ0 : P0 (FZ n0) => fun PS0 : forall i' : FinSet n0, P0 (FS n0 i') => PZ0
+    | FS n0 i' => fun P0 : FinSet (S n0) -> Type => fun PZ0 : P0 (FZ n0) => fun PS0 : forall i' : FinSet n0, P0 (FS n0 i') => PS0 i'
+    end P PZ PS
+  .
+
+  Definition FinSet_rectS {P : forall n : nat, FinSet n -> Type} : (forall n : nat, P (S n) (FZ n)) -> (forall n : nat, forall i' : FinSet n, P n i' -> P (S n) (FS n i')) -> (forall n : nat, forall i : FinSet (S n), P (S n) i) :=
+    fun PZ : forall n : nat, P (S n) (FZ n) =>
+    fun PS : forall n : nat, forall i' : FinSet n, P n i' -> P (S n) (FS n i') =>
+    fix FinSet_rectS_fix (n : nat) (i : FinSet (S n)) {struct i} : P (S n) i :=
+    match i as i0 in FinSet Sn0 return P Sn0 i0 with
+    | FZ n0 => PZ n0
+    | FS n0 i' =>
+      match n0 as n1 return forall i0' : FinSet n1, P (S n1) (FS n1 i0') with
+      | 0 => fun i0' : FinSet 0 => @FinSet_case0 (fun i1 : FinSet 0 => P 1 (FS 0 i1)) i0'
+      | S n0' => fun i0' : FinSet (S n0') => PS (S n0') i0' (FinSet_rectS_fix n0' i0')
+      end i'
+    end
+  .
+
+
+  Lemma forallb_true_iff {A : Type} {p : A -> bool} (xs : list A) :
+    forallb p xs = true <-> forall x : A, In x xs -> p x = true.
+  Proof with try now firstorder.
+    induction xs; simpl...
+    rewrite andb_true_iff.
+    split...
+    intros H0 x H1.
+    destruct H0; destruct H1...
+    rewrite H1 in H...
+  Qed.
+
+  Definition fold_right_max_0 : list nat -> nat :=
+    fold_right max 0
+  .
+
+  Lemma fold_right_max_0_in :
+    forall ns : list nat,
+    forall n : nat,
+    In n ns ->
+    fold_right_max_0 ns >= n.
+  Proof with (lia || eauto).
+    unfold fold_right_max_0.
+    induction ns as [| n' ns]; simpl...
+    intros n H.
+    destruct H...
+    enough (fold_right max 0 ns >= n)...
+  Qed.
+
+  Lemma fold_right_max_0_app :
+    forall ns1 : list nat,
+    forall ns2 : list nat,
+    fold_right_max_0 (ns1 ++ ns2) = max (fold_right_max_0 ns1) (fold_right_max_0 ns2).
+  Proof with (lia || eauto).
+    unfold fold_right_max_0.
+    induction ns1 as [| n1 ns1]; simpl... 
+    intros n.
+    rewrite IHns1...
+  Qed.
+
+  Lemma property1_of_fold_right_max_0 (Phi : nat -> Prop) (Phi_dec : forall i : nat, {Phi i} + {~ Phi i}) :
+    forall ns : list nat,
+    (forall i : nat, Phi i -> In i ns) ->
+    forall n : nat,
+    Phi n ->
+    fold_right max 0 ns >= n.
+  Proof with (lia || eauto).
+    induction ns; simpl.
+    - intros H n H0.
+      contradiction (H n).
+    - intros H n H0.
+      destruct (Compare_dec.le_lt_dec n a)...
+      enough (fold_right max 0 ns >= n)...
+      destruct (Phi_dec n).
+      + destruct (H n p)...
+        enough (forall ks : list nat, forall k : nat, In k ks -> fold_right max 0 ks >= k) by firstorder.
+        induction ks; simpl...
+        intros k H2.
+        destruct H2...
+        enough (fold_right Init.Nat.max 0 ks >= k)...
+      + apply IHns...
+        intros.
+        destruct (H i H1)...
+        subst.
+        contradiction.
+  Qed.
+
+  Lemma property2_of_fold_right_max_0 :
+    forall ns : list nat,
+    forall n : nat,
+    fold_right max 0 ns > n <-> (exists i : nat, In i ns /\ i > n).
+  Proof with (lia || eauto).
+    induction ns; simpl.
+    - split...
+      now firstorder.
+    - intros n.
+      destruct (Compare_dec.le_lt_dec a (fold_right Init.Nat.max 0 ns)); split...
+      + intros H.
+        assert (H0 : fold_right Init.Nat.max 0 ns > n)...
+        destruct (proj1 (IHns n) H0) as [i].
+        now firstorder.
+      + intros H.
+        destruct H as [i].
+        destruct H.
+        destruct H.
+        * subst...
+        * enough (fold_right max 0 ns > n)...
+          apply IHns...
+      + intros H.
+        exists a...
+      + intros H.
+        destruct H as [i].
+        destruct H.
+        destruct H.
+        * subst...
+        * enough (fold_right Init.Nat.max 0 ns > n)...
+          apply IHns...
+  Qed.
+
+  Lemma property3_of_fold_right_max_0 :
+    forall ns1 : list nat,
+    forall ns2 : list nat,
+    fold_right max 0 (ns1 ++ ns2) = max (fold_right max 0 ns1) (fold_right max 0 ns2).
+  Proof.
+    apply fold_right_max_0_app.
+  Qed.
+
+  Lemma property4_of_fold_right_max_0 :
+    forall ns : list nat,
+    forall n : nat,
+    In n ns ->
+    fold_right max 0 ns >= n.
+  Proof with (lia || eauto).
+    induction ns; simpl...
+    intros n H.
+    destruct H...
+    enough (fold_right max 0 ns >= n)...
+  Qed.
+
+  Lemma property5_of_fold_right_max_0 :
+    forall ns1 : list nat,
+    forall ns2 : list nat,
+    (forall n : nat, In n ns1 -> In n ns2) ->
+    fold_right max 0 ns1 <= fold_right max 0 ns2.
+  Proof with (lia || eauto).
+    induction ns1; simpl...
+    intros ns2 H.
+    destruct (Compare_dec.le_lt_dec a (fold_right max 0 ns1)).
+    - enough (fold_right max 0 ns1 <= fold_right max 0 ns2)...
+    - enough (a <= fold_right max 0 ns2)...
+      apply property4_of_fold_right_max_0...
+  Qed.
+
+  Lemma fold_right_max_0_ext :
+    forall ns1 : list nat,
+    forall ns2 : list nat,
+    (forall n : nat, In n ns1 <-> In n ns2) ->
+    fold_right max 0 ns1 = fold_right max 0 ns2.
+  Proof with try now firstorder.
+    intros.
+    enough (fold_right max 0 ns1 <= fold_right max 0 ns2 /\ fold_right max 0 ns2 <= fold_right max 0 ns1) by lia.
+    split; apply property5_of_fold_right_max_0...
+  Qed.
+
+End MyUtilities.
+
+Module MyStructures.
+
+  Class isPoset (A : Type) : Type :=
+    { leProp : A -> A -> Prop
+    ; Poset_requiresPreOrder :> PreOrder leProp
+    ; Poset_requiresPartialOrder :> PartialOrder (@eq A) leProp
+    }
+  .
+
+  Global Hint Resolve Poset_requiresPreOrder : my_hints.
+
+  Global Hint Resolve Poset_requiresPartialOrder : my_hints.
+
+  Global Notation "x =< y" := (leProp x y) (at level 70, no associativity) : type_scope.
+
+  Lemma Poset_refl {A : Type} `{A_isPoset : isPoset A} :
+    forall x : A,
+    x =< x.
+  Proof.
+    apply Poset_requiresPreOrder.
+  Qed.
+
+  Global Hint Resolve Poset_refl : my_hints.
+
+  Lemma Poset_refl1 {A : Type} `{A_isPoset : isPoset A} :
+    forall x1 : A,
+    forall x2 : A,
+    x1 = x2 ->
+    x1 =< x2.
+  Proof.
+    apply Poset_requiresPartialOrder.
+  Qed.
+
+  Global Hint Resolve Poset_refl1 : my_hints.
+
+  Lemma Poset_refl2 {A : Type} `{A_isPoset : isPoset A} :
+    forall x1 : A,
+    forall x2 : A,
+    x1 = x2 ->
+    x2 =< x1.
+  Proof.
+    apply Poset_requiresPartialOrder.
+  Qed.
+
+  Global Hint Resolve Poset_refl2 : my_hints.
+
+  Lemma Poset_asym {A : Type} `{A_isPoset : isPoset A} :
+    forall x1 : A,
+    forall x2 : A,
+    x1 =< x2 ->
+    x2 =< x1 ->
+    x1 = x2.
+  Proof.
+    intros x1 x2 H H0.
+    apply Poset_requiresPartialOrder.
+    split; [apply H | apply H0].
+  Qed.
+
+  Global Hint Resolve Poset_asym : my_hints.
+
+  Lemma Poset_trans {A : Type} `{A_isPoset : isPoset A} :
+    forall x1 : A,
+    forall x2 : A,
+    forall x3 : A,
+    x1 =< x2 ->
+    x2 =< x3 ->
+    x1 =< x3.
+  Proof.
+    apply Poset_requiresPreOrder.
+  Qed.
+
+  Global Hint Resolve Poset_trans : my_hints.
+
+  Global Program Instance nat_isPoset : isPoset nat :=
+    { leProp := le
+    }
+  .
+
+End MyStructures.
+
+Module MyEnsemble.
+
+  Import ListNotations.
+
+  Import MyStructures.
+
+  Definition ensemble : Type -> Type :=
+    fun A : Type =>
+    arrow A Prop
+  .
+
+  Definition member {A : Type} : A -> ensemble A -> Prop :=
+    fun x : A =>
+    fun xs : ensemble A =>
+    xs x
+  .
+
+  Global Hint Unfold member : my_hints.
+
+  Global Notation "x '\in' xs" := (member x xs) (at level 70, no associativity) : type_scope.
+
+  Definition isSubsetOf {A : Type} : ensemble A -> ensemble A -> Prop :=
+    fun xs1 : ensemble A =>
+    fun xs2 : ensemble A =>
+    forall x : A,
+    member x xs1 ->
+    member x xs2
+  .
+
+  Global Hint Unfold isSubsetOf : my_hints.
+
+  Global Notation "xs1 '\subseteq' xs2" := (isSubsetOf xs1 xs2) (at level 70, no associativity) : type_scope.
+
+  Global Program Instance ensemble_isPoset {A : Type} : isPoset (ensemble A) :=
+    { leProp := isSubsetOf
+    }
+  .
+
+  Next Obligation with eauto with *.
+    split...
+  Qed.
+
+  Next Obligation with eauto with *.
+    intros xs1 xs2.
+    split.
+    - repeat red.
+      split.
+      + subst...
+      + red.
+        subst...
+    - intros [H H0].
+      apply functional_extensionality.
+      intros x.
+      apply propositional_extensionality.
+      split.
+      + apply (H x).
+      + apply (H0 x).
+  Qed.
+
+  Inductive finite {A : Type} : list A -> ensemble A :=
+  | in_finite {x : A} :
+    forall xs : list A,
+    In x xs ->
+    member x (finite xs)
+  .
+
+  Global Hint Constructors finite : my_hints.
+
+  Definition empty {A : Type} : ensemble A :=
+    finite []
+  .
+
+  Lemma in_empty_iff {A : Type} :
+    forall x : A,
+    member x empty <-> False.
+  Proof with eauto with *.
+    intros x.
+    split...
+    intros H.
+    inversion H; subst...
+  Qed.
+
+  Global Hint Resolve in_empty_iff : my_hints.
+
+  Definition singleton {A : Type} : A -> ensemble A :=
+    fun x : A => finite [x]
+  .
+
+  Lemma in_singleton_iff {A : Type} :
+    forall x : A,
+    forall x1 : A,
+    member x (singleton x1) <-> x1 = x.
+  Proof with eauto with *.
+    intros x x1.
+    split.
+    - intros H.
+      inversion H; subst.
+      destruct H0 as [H0 | []]...
+    - intros H.
+      subst...
+  Qed.
+
+  Global Hint Resolve in_singleton_iff : my_hints.
+
+  Inductive unions {A : Type} : ensemble (ensemble A) -> ensemble A :=
+  | in_unions {x : A} :
+    forall xs : ensemble A,
+    forall xss : ensemble (ensemble A),
+    member x xs ->
+    member xs xss ->
+    member x (unions xss)
+  .
+
+  Global Hint Constructors unions : my_hints.
+
+  Definition union {A : Type} : ensemble A -> ensemble A -> ensemble A :=
+    fun xs1 : ensemble A =>
+    fun xs2 : ensemble A =>
+    unions (finite [xs1; xs2])
+  .
+
+  Lemma in_union_iff {A : Type} :
+    forall xs1 : ensemble A,
+    forall xs2 : ensemble A,
+    forall x : A,
+    member x (union xs1 xs2) <-> (member x xs1 \/ member x xs2).
+  Proof with eauto with *.
+    intros xs1 xs2 x.
+    split.
+    - intros H.
+      inversion H; subst.
+      inversion H1; subst.
+      destruct H2 as [H2 | [H2 | []]]; subst...
+    - intros [H | H]; [apply (in_unions xs1) | apply (in_unions xs2)]...
+  Qed.
+
+  Global Hint Resolve in_union_iff : my_hints.
+
+  Inductive intersection {A : Type} : ensemble A -> ensemble A -> ensemble A :=
+  | in_intersection {x : A} :
+    forall xs1 : ensemble A,
+    forall xs2 : ensemble A,
+    member x xs1 ->
+    member x xs2 ->
+    member x (intersection xs1 xs2)
+  .
+
+  Global Hint Constructors intersection : my_hints.
+
+  Inductive full {A : Type} : ensemble A :=
+  | in_full {x : A} :
+    member x full
+  .
+
+  Global Hint Constructors full : my_hints.
+
+  Inductive image {A : Type} {B : Type} : (A -> B) -> ensemble A -> ensemble B :=
+  | in_image {x : A} :
+    forall f : A -> B,
+    forall xs : ensemble A,
+    member x xs ->
+    member (f x) (image f xs)
+  .
+
+  Global Hint Constructors image : my_hints.
+
+  Inductive preimage {A : Type} {B : Type} : (A -> B) -> ensemble B -> ensemble A :=
+  | in_preimage {x : A} :
+    forall f : A -> B,
+    forall ys : ensemble B,
+    member (f x) ys ->
+    member x (preimage f ys)
+  .
+
+  Global Hint Constructors preimage : my_hints.
+
+  Definition nonempty {A : Type} : ensemble A -> Prop :=
+    fun xs : ensemble A =>
+    exists x : A, member x xs
+  .
+
+  Global Hint Unfold nonempty : my_hints.
+
+End MyEnsemble.
+
+Module GeneralTopology.
 
 Import ListNotations.
 
-Import AuxiliaryPalatina.
+Import MyStructures.
 
-Import DomainTheory.
+Import MyEnsemble.
 
-Definition ivar : Set :=
-  nat
+Class isTopologicalSpace (X : Type) : Type :=
+  { isOpen : ensemble X -> Prop
+  ; open_for_full :
+    isOpen full
+  ; open_for_unions :
+    forall xss : ensemble (ensemble X),
+    (forall xs : ensemble X, member xs xss -> isOpen xs) ->
+    isOpen (unions xss)
+  ; open_for_intersection :
+    forall xs1 : ensemble X,
+    forall xs2 : ensemble X,
+    isOpen xs1 ->
+    isOpen xs2 ->
+    isOpen (intersection xs1 xs2)
+  }
 .
 
-Definition ivar_eq_dec :
-  forall x : ivar,
-  forall y : ivar,
-  {x = y} + {x <> y}.
-Proof.
-  apply Nat.eq_dec.
-Defined.
+Global Hint Resolve open_for_full : my_hints.
 
-Inductive tm : Set :=
-| tmVar : forall x : ivar, tm
-| tmApp : forall P1 : tm, forall P2 : tm, tm
-| tmLam : forall y : ivar, forall Q : tm, tm
+Global Hint Resolve open_for_unions : my_hints.
+
+Global Hint Resolve open_for_intersection : my_hints.
+
+Definition isContinuousMap {X : Type} {Y : Type} `{X_isTopologicalSpace : isTopologicalSpace X} `{Y_isTopologicalSpace : isTopologicalSpace Y} : (X -> Y) -> Prop :=
+  fun f : X -> Y =>
+  forall ys : ensemble Y,
+  isOpen ys ->
+  isOpen (preimage f ys)
 .
 
-Definition tm_eq_dec :
-  forall M1 : tm,
-  forall M2 : tm,
-  {M1 = M2} + {M1 <> M2}.
-Proof with try ((left; congruence) || (right; congruence)).
-  induction M1; destruct M2...
-  - destruct (ivar_eq_dec x x0)...
-  - destruct (IHM1_1 M2_1); destruct (IHM1_2 M2_2)...
-  - destruct (ivar_eq_dec y y0); destruct (IHM1 M2)...
-Defined.
+Global Hint Unfold isContinuousMap : my_hints.
 
-Section Subterm.
+End GeneralTopology.
 
-Fixpoint getRank (M : tm) {struct M} : nat :=
-  match M with
-  | tmVar x => 0
-  | tmApp P1 P2 => S (max (getRank P1) (getRank P2))
-  | tmLam y Q => S (getRank Q)
-  end
-.
+Module DomainTheory.
 
-Inductive subtm : tm -> tm -> Set :=
-| subtmRefl : forall M : tm, subtm M M
-| subtmAppL : forall M : tm, forall P1 : tm, forall P2 : tm, subtm M P1 -> subtm M (tmApp P1 P2)
-| subtmAppR : forall M : tm, forall P1 : tm, forall P2 : tm, subtm M P2 -> subtm M (tmApp P1 P2)
-| subtmLAbs : forall M : tm, forall y : ivar, forall Q : tm, subtm M Q -> subtm M (tmLam y Q)
-.
+  Import ListNotations.
 
-Local Hint Constructors tm : core.
+  Import MyStructures.
 
-Lemma subtm_getRank :
-  forall M : tm,
-  forall N : tm,
-  subtm M N ->
-  getRank M <= getRank N.
-Proof with lia.
-  intros M N X.
-  induction X; simpl...
-Qed.
+  Import MyEnsemble.
 
-Lemma subtm_and_same_rank_implies_same_term :
-  forall M : tm,
-  forall N : tm,
-  subtm M N ->
-  getRank M = getRank N ->
-  M = N.
-Proof with lia.
-  intros M N X.
-  destruct X; intros.
-  - reflexivity.
-  - assert (H0 := subtm_getRank M P1 X).
-    simpl in *...
-  - assert (H0 := subtm_getRank M P2 X).
-    simpl in *...
-  - assert (H0 := subtm_getRank M Q X).
-    simpl in *...
-Qed.
+  Import GeneralTopology.
 
-Lemma subtm_refl :
-  forall M1 : tm,
-  subtm M1 M1.
-Proof.
-  apply subtmRefl.
-Qed.
+  Definition isSupremum {D : Type} `{D_isPoset : isPoset D} : D -> ensemble D -> Prop :=
+    fun sup_X : D =>
+    fun X : ensemble D =>
+    forall d : D,
+    sup_X =< d <-> (forall x : D, member x X -> x =< d)
+  .
 
-Local Hint Resolve subtm_refl : core.
+  Global Hint Unfold isSupremum : my_hints.
 
-Lemma subtm_asym :
-  forall M1 : tm,
-  forall M2 : tm,
-  subtm M1 M2 ->
-  subtm M2 M1 ->
-  M1 = M2.
-Proof with eauto.
-  intros.
-  apply subtm_and_same_rank_implies_same_term...
-  enough (getRank M1 <= getRank M2 /\ getRank M2 <= getRank M1) by lia.
-  split; apply subtm_getRank...
-Qed.
+  Lemma isSupremum_upperbound {D : Type} `{D_isPoset : isPoset D} :
+    forall sup_X : D,
+    forall X : ensemble D,
+    isSupremum sup_X X ->
+    forall x : D,
+    member x X ->
+    x =< sup_X.
+  Proof with eauto with *.
+    intros sup_X X H x H0.
+    apply H...
+  Qed.
 
-Local Hint Resolve subtm_asym : core.
+  Global Hint Resolve isSupremum_upperbound : my_hints.
 
-Lemma subtm_trans :
-  forall M1 : tm,
-  forall M2 : tm,
-  forall M3 : tm,
-  subtm M1 M2 ->
-  subtm M2 M3 ->
-  subtm M1 M3.
-Proof with eauto.
-  enough (claim1 : forall L : tm, forall N : tm, forall M : tm, subtm N L -> subtm M N -> subtm M L)...
-  induction L.
-  all: intros; inversion H; subst...
-  - constructor 2...
-  - constructor 3...
-  - constructor 4...
-Qed.
+  Lemma isSupremum_isSubsetOf {D : Type} `{D_isPoset : isPoset D} :
+    forall X1 : ensemble D,
+    forall X2 : ensemble D,
+    isSubsetOf X1 X2 ->
+    forall sup_X1 : D,
+    isSupremum sup_X1 X1 ->
+    forall sup_X2 : D,
+    isSupremum sup_X2 X2 ->
+    sup_X1 =< sup_X2.
+  Proof with eauto with *.
+    intros X1 X2 H sup_X1 H0 sup_X2 H1.
+    apply H0...
+  Qed.
 
-Local Hint Resolve subtm_trans : core.
+  Global Hint Resolve isSupremum_isSubsetOf : my_hints.
 
-Theorem strong_induction_on_tm (phi : tm -> Prop) :
-  (forall M : tm, (forall N : tm, subtm N M -> N <> M -> phi N) -> phi M) ->
-  forall M : tm,
-  phi M.
-Proof with try now (firstorder; eauto).
-  intros XXX.
-  enough (claim1 : forall M : tm, forall L : tm, subtm L M -> phi L)...
-  induction M.
-  all: intros L H; apply XXX; intros N H0 H1; inversion H0; subst...
-  all: inversion H; subst...
-Qed.
+  Lemma isSupremum_ext {D : Type} `{D_isPoset : isPoset D} :
+    forall X1 : ensemble D,
+    forall X2 : ensemble D,
+    (forall x : D, member x X1 <-> member x X2) ->
+    forall sup_X1 : D,
+    isSupremum sup_X1 X1 ->
+    forall sup_X2 : D,
+    isSupremum sup_X2 X2 <-> sup_X1 = sup_X2.
+  Proof with eauto with *.
+    intros X1 X2 H sup_X1 H0 sup_X2.
+    assert (claim1 := fun x : D => fun H1 : member x X1 => proj1 (H x) H1).
+    assert (claim2 := fun x : D => fun H1 : member x X2 => proj2 (H x) H1).
+    split...
+    intros H1.
+    intros x.
+    split.
+    - intros H2 x' H3.
+      apply H0...
+    - intros H2.
+      enough (H3 : sup_X1 =< x) by apply (Poset_trans sup_X2 sup_X1 x (Poset_refl2 sup_X1 sup_X2 H1) H3).
+      apply H0...
+  Qed.
 
-End Subterm.
+  Global Hint Resolve isSupremum_ext : my_hints.
 
-Section Occurences.
+  Lemma isSupremum_unique {D : Type} `{D_isPoset : isPoset D} :
+    forall X : ensemble D,
+    forall sup1 : D,
+    isSupremum sup1 X ->
+    forall sup2 : D,
+    isSupremum sup2 X <-> sup1 = sup2.
+  Proof with eauto with *.
+    intros X sup1 H sup2...
+  Qed.
 
-Definition occurence_rect (XP : forall z : ivar, forall M : tm, subtm (tmVar z) M -> Type) :
-  (forall x : ivar, XP x (tmVar x) (subtmRefl (tmVar x))) ->
-  (forall x : ivar, forall P1 : tm, forall P2 : tm, forall X : subtm (tmVar x) P1, XP x P1 X -> XP x (tmApp P1 P2) (subtmAppL (tmVar x) P1 P2 X)) ->
-  (forall x : ivar, forall P1 : tm, forall P2 : tm, forall X : subtm (tmVar x) P2, XP x P2 X -> XP x (tmApp P1 P2) (subtmAppR (tmVar x) P1 P2 X)) ->
-  (forall x : ivar, forall y : ivar, forall Q : tm, forall X : subtm (tmVar x) Q, XP x Q X -> XP x (tmLam y Q) (subtmLAbs (tmVar x) y Q X)) ->
-  (forall x : ivar, forall M : tm, forall X : subtm (tmVar x) M, XP x M X).
-Proof.
-  intros XP_refl XP_appl XP_appr XP_labs z.
-  assert ( XXX :
-    forall N : tm,
+  Global Hint Resolve isSupremum_unique : my_hints.
+
+    Definition image_sup {D : Type} `{D_isPoset : isPoset D} : ensemble (ensemble D) -> ensemble D :=
+      fun Xs : ensemble (ensemble D) =>
+      fun sup_X : D =>
+      exists X : ensemble D, member X Xs /\ isSupremum sup_X X
+    .
+
+  Global Hint Unfold image_sup : my_hints.
+
+  Lemma sup_image_sup_isGreaterThan {D : Type} `{D_isPoset : isPoset D} :
+    forall Xs : ensemble (ensemble D),
+    forall sup : D,
+    isSupremum sup (image_sup Xs) ->
+    forall X : ensemble D,
+    member X Xs ->
+    forall sup_X : D,
+    isSupremum sup_X X ->
+    sup_X =< sup.
+  Proof with eauto with *.
+    intros Xs sup H X H0 sup_X H1.
+    apply H...
+  Qed.
+
+  Global Hint Resolve sup_image_sup_isGreaterThan : my_hints.
+
+  Lemma isSupremum_unions_Xs_iff_isSupremum_image_sup_Xs {D : Type} `{D_isPoset : isPoset D} :
+    forall Xs : ensemble (ensemble D),
+    (forall X : ensemble D, member X Xs -> exists sup_X : D, isSupremum sup_X X) ->
+    forall sup : D,
+    isSupremum sup (unions Xs) <-> isSupremum sup (image_sup Xs).
+  Proof with eauto with *.
+    intros Xs H sup.
+    split.
+    - intros H0 x.
+      split.
+      + intros H1 x' [X [H2 H3]].
+        apply H3...
+      + intros H1.
+        apply H0.
+        intros x' H2.
+        inversion H2; subst.
+        destruct (H xs H4) as [sup_xs H5].
+        apply H5...
+        apply H1...
+    - intros H0 x.
+      split.
+      + intros H1 x' H2.
+        inversion H2; subst.
+        destruct (H xs H4) as [sup_xs H5].
+        apply H5...
+      + intros H1.
+        apply H0.
+        intros x' [X [H2 H3]].
+        apply H3...
+  Qed.
+
+  Class isCompleteLattice (D : Type) : Type :=
+    { CompleteLattice_requiresPoset :> isPoset D
+    ; supremum_always_exists :
+      forall X : ensemble D,
+      {sup_X : D | isSupremum sup_X X}
+    }
+  .
+
+  Global Hint Resolve supremum_always_exists : my_hints.
+
+  Lemma unions_isSupremum {A : Type} :
+    forall Xs : ensemble (ensemble A),
+    isSupremum (unions Xs) Xs.
+  Proof with eauto with *.
+    intros Xs X.
+    split.
+    - intros H xs H0.
+      transitivity (unions Xs)...
+      intros x H1.
+      apply (in_unions xs)...
+    - intros H x H0.
+      inversion H0; subst.
+      apply (H xs)...
+  Qed.
+
+  Global Instance ensemble_isCompleteLattice {A : Type} : isCompleteLattice (ensemble A) :=
+    { CompleteLattice_requiresPoset := ensemble_isPoset
+    ; supremum_always_exists :=
+      fun Xs : ensemble (ensemble A) =>
+      exist _ (unions Xs) (unions_isSupremum Xs)
+    }
+  .
+
+  Definition isDirected {D : Type} `{D_isPoset : isPoset D} : ensemble D -> Prop :=
+    fun X : ensemble D =>
+    nonempty X /\ (forall x1 : D, member x1 X -> forall x2 : D, member x2 X -> exists x3 : D, member x3 X /\ x1 =< x3 /\ x2 =< x3)
+  .
+
+  Global Hint Unfold isDirected : my_hints.
+
+  Class isCompletePartialOrder (D : Type) : Type :=
+    { CompletePartialOrder_requiresPoset :> isPoset D
+    ; bottom_exists : {min_D : D | forall x : D, min_D =< x}
+    ; square_up_exists :
+      forall X : ensemble D,
+      isDirected X ->
+      {sup_X : D | isSupremum sup_X X}
+    }
+  .
+
+  Global Program Instance CompleteLattice_isCompletePartialOrder {D : Type} (D_requiresCompleteLattice : isCompleteLattice D) : isCompletePartialOrder D :=
+    { CompletePartialOrder_requiresPoset := CompleteLattice_requiresPoset
+    }
+  .
+
+  Next Obligation.
+    destruct (supremum_always_exists empty) as [min_D H].
+    exists min_D.
+    intros x.
+    apply H.
+    intros x' H0.
+    inversion H0; subst.
+    inversion H1.
+  Defined.
+
+  Next Obligation.
+    apply supremum_always_exists.
+  Defined.
+
+  Global Program Instance ScottTopology_isTopologicalSpace {D : Type} (D_requiresCompletePartialOrder : isCompletePartialOrder D) : isTopologicalSpace D :=
+    { isOpen :=
+      fun O : ensemble D =>
+      (forall x : D, forall y : D, member x O -> x =< y -> member y O) /\ (forall X : ensemble D, isDirected X -> forall sup_X : D, isSupremum sup_X X -> member sup_X O -> nonempty (intersection X O))
+    }
+  .
+
+  Next Obligation with eauto with *.
+    split...
+    intros.
+    destruct H as [[x H] H2]...
+  Qed.
+
+  Next Obligation with eauto with *.
+    split.
+    - intros.
+      destruct H0.
+      apply (in_unions xs)...
+      apply (proj1 (H xs H2) x y)...
+    - intros.
+      inversion H0; subst.
+      inversion H2; subst.
+      destruct (proj2 (H xs H6) X H0 sup_X H1 H5) as [x H7].
+      inversion H7; subst...
+  Qed.
+
+  Next Obligation with eauto with *.
+    split.
+    - intros.
+      destruct H3...
+    - intros.
+      inversion H5; subst.
+      destruct (H2 X H3 sup_X H4 H6) as [x1 H8].
+      destruct (H1 X H3 sup_X H4 H7) as [x2 H9].
+      inversion H3; subst.
+      inversion H8; inversion H9; subst.
+      destruct (H11 x1 H12 x2 H17) as [x [H14 [H15 H16]]].
+      exists x...
+  Qed.
+
+  Definition U {D : Type} `{D_isCompletePartialOrder : isCompletePartialOrder D} : D -> ensemble D :=
+    fun x : D =>
+    fun z : D =>
+    ~ z =< x
+  .
+
+  Global Hint Unfold U : my_hints.
+
+  Lemma U_x_isOpen {D : Type} `{D_isCompletePartialOrder : isCompletePartialOrder D} :
+    forall x : D,
+    isOpen (U x).
+  Proof with eauto with *.
+    intros x.
+    assert ( claim1 :
+      forall y : D,
+      forall z : D,
+      member y (U x) ->
+      y =< z ->
+      member z (U x)
+    ).
+    { intros y z H H0 H1.
+      contradiction H...
+    }
+    split...
+    intros X H sup_X H0 H1.
+    inversion H; subst.
+    assert (claim2 : ~ (forall x0 : D, x0 =< x \/ ~ member x0 X)).
+    { intros H4.
+      contradiction H1.
+      apply (proj2 (H0 x)).
+      intros x0 H5.
+      destruct (H4 x0); [apply H6 | contradiction].
+    }
+    apply not_all_ex_not in claim2.
+    destruct claim2 as [x1 H4].
+    exists x1.
+    apply not_or_and in H4.
+    destruct H4 as [H4 H5].
+    apply NNPP in H5...
+  Qed.
+
+  Definition characterization_of_ContinuousMap_on_cpos {D : Type} {D' : Type} `{D_isCompletePartialOrder : isCompletePartialOrder D} `{D'_isCompletePartialOrder : isCompletePartialOrder D'} : (D -> D') -> Prop :=
+    fun f : D -> D' =>
+    forall X : ensemble D,
+    isDirected X ->
+    let Y : ensemble D' := image f X in
+    exists sup_X : D, exists sup_Y : D', isSupremum sup_X X /\ isSupremum sup_Y Y /\ f sup_X = sup_Y
+  .
+
+  Lemma ContinuousMaps_on_cpos_are_always_monotonic {D : Type} {D' : Type} `{D_isCompletePartialOrder : isCompletePartialOrder D} `{D'_isCompletePartialOrder : isCompletePartialOrder D'} :
+    forall f : D -> D',
+    isContinuousMap f ->
+    forall x1 : D,
+    forall x2 : D,
+    x1 =< x2 ->
+    f x1 =< f x2.
+  Proof with eauto with *.
+    intros f H x1 x2 H0.
+    apply NNPP.
+    intros H1.
+    assert (H2 : member (f x1) (U (f x2))) by now unfold U.
+    assert (H3 : member x1 (preimage f (U (f x2)))) by now constructor.
+    assert (H4 : isOpen (preimage f (U (f x2)))) by now apply H, U_x_isOpen.
+    assert (H5 : member x2 (preimage f (U (f x2)))) by now apply (proj1 H4 x1 x2).
+    enough (H6 : member (f x2) (U (f x2)))...
+    inversion H5...
+  Qed.
+
+  Lemma ContinuousMaps_preservesDirected {D : Type} {D' : Type} `{D_isCompletePartialOrder : isCompletePartialOrder D} `{D'_isCompletePartialOrder : isCompletePartialOrder D'} :
+    forall f : D -> D',
+    isContinuousMap f ->
+    forall X : ensemble D,
+    isDirected X ->
+    isDirected (image f X).
+  Proof with eauto with *.
+    intros f H X H0.
+    destruct H0 as [H0 H1].
+    assert (H2 : forall x1 : D, forall x2 : D, x1 =< x2 -> f x1 =< f x2) by now apply ContinuousMaps_on_cpos_are_always_monotonic.
+    split.
+    - destruct H0 as [x0 H0]...
+    - intros y1 H3 y2 H4.
+      inversion H3; inversion H4; subst.
+      rename x into x1, x0 into x2.
+      destruct (H1 x1 H5 x2 H9) as [x3 [H6 [H7 H8]]].
+      exists (f x3).
+      repeat split...
+  Qed.
+
+  Lemma ContinuousMaps_preservesSupremum {D : Type} {D' : Type} `{D_isCompletePartialOrder : isCompletePartialOrder D} `{D'_isCompletePartialOrder : isCompletePartialOrder D'} :
+    forall f : D -> D',
+    isContinuousMap f ->
+    forall X : ensemble D,
+    isDirected X ->
+    forall sup_X : D,
+    isSupremum sup_X X ->
+    isDirected (image f X) ->
+    {sup_Y : D' | isSupremum sup_Y (image f X) /\ f sup_X = sup_Y}.
+  Proof with eauto with *.
+    intros f H X H0 sup_X H1 H2.
+    set (Y := image f X).
+    assert (H3 : forall x1 : D, forall x2 : D, x1 =< x2 -> f x1 =< f x2) by now apply ContinuousMaps_on_cpos_are_always_monotonic.
+    destruct (square_up_exists Y H2) as [sup_Y H4].
+    exists sup_Y.
+    assert (claim1 : sup_Y =< f sup_X).
+    { apply H4.
+      intros y H5.
+      inversion H5; subst.
+      apply H3, H1...
+    }
+    assert (claim2 : f sup_X =< sup_Y).
+    { apply NNPP.
+      intros H5.
+      assert (H6 : member (f sup_X) (U sup_Y)) by now unfold U.
+      assert (H7 : member sup_X (preimage f (U sup_Y))) by now constructor.
+      assert (H8 : isOpen (preimage f (U sup_Y))) by now apply H, U_x_isOpen.
+      destruct H8.
+      destruct (H9 X H0 sup_X H1 H7) as [x1 H10].
+      inversion H10; subst.
+      inversion H12; subst.
+      contradiction H13...
+    }
+    split...
+  Qed.
+
+  Theorem the_main_reason_for_introducing_ScottTopology {D : Type} {D' : Type} `{D_isCompletePartialOrder : isCompletePartialOrder D} `{D'_isCompletePartialOrder : isCompletePartialOrder D'} :
+    forall f : D -> D',
+    isContinuousMap f <-> characterization_of_ContinuousMap_on_cpos f.
+  Proof with eauto with *.
+    assert (claim1 : forall f : D -> D', isContinuousMap f -> forall x1 : D, forall x2 : D, x1 =< x2 -> f x1 =< f x2) by apply ContinuousMaps_on_cpos_are_always_monotonic.
+    split.
+    - intros H X H0.
+      inversion H0; subst.
+      set (Y := image f X).
+      assert (H3 : isDirected Y) by now apply ContinuousMaps_preservesDirected.
+      destruct (square_up_exists X H0) as [sup_X H4].
+      exists sup_X.
+      destruct (ContinuousMaps_preservesSupremum f H X H0 sup_X H4 H3) as [sup_Y H5].
+      exists sup_Y...
+    - intros H.
+      assert (claim2 : forall x1 : D, forall x2 : D, x1 =< x2 -> f x1 =< f x2).
+      { intros x1 x2 H0.
+        set (X := finite [x1; x2]).
+        set (Y := image f X).
+        assert (H1 : isSupremum x2 X).
+        { intros x.
+          split.
+          - intros H1 x' H2.
+            inversion H2; subst.
+            destruct H3 as [H3 | [H3 | []]]...
+          - intros H1...
+        }
+        assert (H2 : isDirected X).
+        { split.
+          - exists x1...
+          - intros x1' H2 x2' H3.
+            exists x2.
+            enough (x1' =< x2 /\ x2' =< x2)...
+        }
+        destruct (H X H2) as [sup_X H3].
+        destruct H3 as [sup_Y [H3 [H4 H5]]].
+        assert (H6 : sup_X = x2) by now apply (isSupremum_unique X).
+        subst...
+      }
+      intros O H0.
+      split.
+      + intros x1 x2 H1 H2.
+        inversion H1; subst.
+        constructor.
+        apply (proj1 H0 (f x1) (f x2))...
+      + intros X H1 sup_X H2 H3.
+        destruct (H X H1) as [sup_X' [sup_Y [H4 [H5 H6]]]].
+        assert (H7 : sup_X = sup_X') by now apply (isSupremum_unique X).
+        subst sup_X' sup_Y.
+        assert (H8 : member (f sup_X) O) by now inversion H3; subst.
+        assert (H9 : isDirected (image f X)).
+        { destruct H1 as [[x1_0 H1] H6].
+          split.
+          - exists (f x1_0)...
+          - intros y1 H10 y2 H11.
+            inversion H10; subst.
+            inversion H11; subst.
+            rename x into x1, x0 into x2.
+            destruct (H6 x1 H7 x2 H9) as [x3 [H12 [H13 H14]]].
+            exists (f x3).
+            repeat split...
+        }
+        assert (H10 : nonempty (intersection (image f X) O)).
+        { apply (proj2 H0 (image f X) H9 (f sup_X))...
+        }
+        destruct H10 as [y1 H10].
+        inversion H10; subst.
+        inversion H6; subst.
+        exists x...
+  Qed.
+
+  Local Program Instance DirectProductOfTwoPosets_isPoset {D : Type} {D' : Type} (D_requiresPoset : isPoset D) (D'_requiresPoset : isPoset D') : isPoset (D * D') :=
+    { leProp :=
+      fun p1 : (D * D') =>
+      fun p2 : (D * D') =>
+      fst p1 =< fst p2 /\ snd p1 =< snd p2
+    }
+  .
+
+  Next Obligation with eauto with *.
+    split.
+    - intros [x1 y1]...
+    - intros [x1 y1] [x2 y2] [x3 y3] [H H0] [H1 H2]...
+  Qed.
+
+  Next Obligation with eauto with *.
+    split.
+    - intros H.
+      subst.
+      repeat red.
+      repeat split...
+    - intros [[H H0] [H1 H2]].
+      apply injective_projections...
+  Qed.
+
+  Inductive getFsts {D : Type} {D' : Type} : ensemble (D * D') -> ensemble D :=
+  | in_getFsts {ps : ensemble (D * D')} :
+    forall x : D,
+    forall x' : D',
+    member (x, x') ps ->
+    member x (getFsts ps)
+  .
+
+  Global Hint Constructors getFsts : domain_theory_hints.
+
+  Inductive getSnds {D : Type} {D' : Type} : ensemble (D * D') -> ensemble D' :=
+  | in_getSnds {ps : ensemble (D * D')} :
+    forall x : D,
+    forall x' : D',
+    member (x, x') ps ->
+    member x' (getSnds ps)
+  .
+
+  Global Hint Constructors getSnds : domain_theory_hints.
+
+  Local Program Instance DirectProductOfTwoCompletePartialOrders_isCompletePartialOrder {D : Type} {D' : Type} (D_requiresCompletePartialOrder : isCompletePartialOrder D) (D'_requiresCompletePartialOrder : isCompletePartialOrder D') : isCompletePartialOrder (D * D') :=
+    { CompletePartialOrder_requiresPoset := DirectProductOfTwoPosets_isPoset (@CompletePartialOrder_requiresPoset D D_requiresCompletePartialOrder) (@CompletePartialOrder_requiresPoset D' D'_requiresCompletePartialOrder)
+    }
+  .
+
+  Next Obligation.
+    destruct (@bottom_exists D D_requiresCompletePartialOrder) as [bot_D H].
+    destruct (@bottom_exists D' D'_requiresCompletePartialOrder) as [bot_D' H0].
+    exists (bot_D, bot_D').
+    intros [d d'].
+    split; [apply H | apply H0].
+  Defined.
+
+  Next Obligation.
+    assert (claim1 : isDirected (getFsts X)).
+    { destruct H as [H H0].
+      split.
+      - destruct H as [[d0 d0'] H].
+        exists d0.
+        apply (in_getFsts d0 d0' H).
+      - intros d1 H1 d2 H2.
+        inversion H1; subst.
+        inversion H2; subst.
+        rename x' into d1', x'0 into d2'.
+        destruct (H0 (d1, d1') H3 (d2, d2') H4) as [[d3 d3'] [H5 [[H6 H7] [H8 H9]]]].
+        exists d3.
+        split.
+        + apply (in_getFsts d3 d3' H5).
+        + split; [apply H6 | apply H8].
+    }
+    assert (claim2 : isDirected (getSnds X)).
+    { destruct H as [H H0].
+      split.
+      - destruct H as [[d0 d0'] H].
+        exists d0'.
+        apply (in_getSnds d0 d0' H).
+      - intros d1' H1 d2' H2.
+        inversion H1; subst.
+        inversion H2; subst.
+        rename x into d1, x0 into d2.
+        destruct (H0 (d1, d1') H3 (d2, d2') H4) as [[d3 d3'] [H5 [[H6 H7] [H8 H9]]]].
+        exists d3'.
+        split.
+        + apply (in_getSnds d3 d3' H5).
+        + split; [apply H7 | apply H9].
+    }
+    destruct (@square_up_exists D D_requiresCompletePartialOrder (getFsts X) claim1) as [sup_X1 H0].
+    destruct (@square_up_exists D' D'_requiresCompletePartialOrder (getSnds X) claim2) as [sup_X2 H1].
+    exists (sup_X1, sup_X2).
+    intros [d d'].
+    split.
+    - intros H2 [x x'] H3.
+      split.
+      + apply H0.
+        * apply (proj1 H2).
+        * apply (in_getFsts x x' H3).
+      + apply H1.
+        * apply (proj2 H2).
+        * apply (in_getSnds x x' H3).
+    - intros H2.
+      split.
+      + apply H0.
+        intros x H3.
+        inversion H3; subst.
+        apply (proj1 (H2 (x, x') H4)).
+      + apply H1.
+        intros x' H3.
+        inversion H3; subst.
+        apply (proj2 (H2 (x, x') H4)).
+  Defined.
+
+  Local Notation "D1 ~> D2" := ({f : D1 -> D2 | isContinuousMap f}) (at level 70, no associativity) : type_scope.
+
+  Definition ContinuousMap_is_continuous {D : Type} {D' : Type} `{D_isCompletePartialOrder : isCompletePartialOrder D} `{D'_isCompletePartialOrder : isCompletePartialOrder D'} : forall f : D ~> D', isContinuousMap (proj1_sig f) :=
+    fun f : D ~> D' => proj2_sig f
+  .
+
+  Global Hint Resolve ContinuousMap_is_continuous : my_hints.
+
+  Lemma squigarrows_are_the_same_iff {D : Type} {D' : Type} `{D_isCompletePartialOrder : isCompletePartialOrder D} `{D'_isCompletePartialOrder : isCompletePartialOrder D'} :
+    forall f1 : D ~> D',
+    forall f2 : D ~> D',
+    (forall x : D, proj1_sig f1 x = proj1_sig f2 x) ->
+    f1 = f2.
+  Proof with eauto.
+    intros f1 f2 H.
+    enough (claim1 : proj1_sig f1 = proj1_sig f2) by apply (eq_sig f1 f2 claim1), proof_irrelevance.
+    apply functional_extensionality...
+  Qed.
+
+  Global Hint Resolve squigarrows_are_the_same_iff : my_hints.
+
+  Local Program Instance squigarrow_isPoset {D : Type} {D' : Type} (D_requiresCompletePartialOrder : isCompletePartialOrder D) (D'_requiresCompletePartialOrder : isCompletePartialOrder D') : isPoset (D ~> D') :=
+    { leProp :=
+      fun f1 : D ~> D' =>
+      fun f2 : D ~> D' =>
+      forall x : D,
+      proj1_sig f1 x =< proj1_sig f2 x
+    }
+  .
+
+  Next Obligation with eauto with *.
+    split...
+  Qed.
+
+  Next Obligation with eauto with *.
+    split.
+    - intros H.
+      subst.
+      split; intros x...
+    - intros [H H0]...
+  Qed.
+
+  Lemma sup_of_squigarrow_is_well_defined {D : Type} {D' : Type} `{D_isCompletePartialOrder : isCompletePartialOrder D} `{D'_isCompletePartialOrder : isCompletePartialOrder D'} :
+    forall fs : ensemble (D ~> D'),
+    isDirected fs ->
+    forall x : D,
+    isDirected (image (fun f : D ~> D' => proj1_sig f x) fs).
+  Proof with eauto with *.
+    intros fs [H H0] x.
+    split.
+    - destruct H as [f0].
+      exists (proj1_sig f0 x).
+      apply (in_image (fun f : D ~> D' => proj1_sig f x))...
+    - intros y1 H1 y2 H2.
+      inversion H1; subst.
+      inversion H2; subst.
+      rename x0 into f1, x1 into f2.
+      destruct (H0 f1 H3 f2 H4) as [f3 [H5 [H6 H7]]].
+      exists (proj1_sig f3 x).
+      repeat split...
+      apply (in_image (fun f : D ~> D' => proj1_sig f x))...
+  Qed.
+
+  Lemma sup_of_set_of_squigarrows_exists_if_it_is_directed {D : Type} {D' : Type} `{D_isCompletePartialOrder : isCompletePartialOrder D} `{D'_isCompletePartialOrder : isCompletePartialOrder D'} :
+    forall fs : ensemble (D ~> D'),
+    forall fs_isDirected : isDirected fs,
+    let f : D -> D' := fun x : D => proj1_sig (square_up_exists (image (fun f_i : D ~> D' => proj1_sig f_i x) fs) (sup_of_squigarrow_is_well_defined fs fs_isDirected x)) in
+    isContinuousMap f.
+  Proof with eauto with *.
+    intros fs H f.
+    apply the_main_reason_for_introducing_ScottTopology.
+    intros X H0 Y.
+    destruct (square_up_exists X H0) as [sup_X H1].
+    exists sup_X, (f sup_X).
+    assert ( claim1 :
+      forall f_i : D ~> D',
+      member f_i fs ->
+      isSupremum (proj1_sig f_i sup_X) (image (fun x : D => proj1_sig f_i x) X)
+    ).
+    { intros f_i H2.
+      assert (H3 : isContinuousMap (proj1_sig f_i))...
+      assert (H4 : characterization_of_ContinuousMap_on_cpos (proj1_sig f_i)) by now apply the_main_reason_for_introducing_ScottTopology.
+      destruct (H4 X H0) as [sup_X' [sup_Y' [H5 [H6 H7]]]].
+      assert (H8 : sup_X' = sup_X) by now apply (isSupremum_unique X).
+      subst...
+    }
+    assert (claim2 : isSupremum (f sup_X) (image (fun f_i : D ~> D' => proj1_sig f_i sup_X) fs)) by apply (proj2_sig (square_up_exists (image (fun f_i : D ~> D' => proj1_sig f_i sup_X) fs) (sup_of_squigarrow_is_well_defined fs H sup_X))).
+    assert (claim3 : isSupremum (f sup_X) (unions (image (fun f_i : D ~> D' => image (fun x : D => proj1_sig f_i x) X) fs))).
+    { apply isSupremum_unions_Xs_iff_isSupremum_image_sup_Xs.
+      - intros ys H2.
+        inversion H2; subst.
+        rename x into f_i.
+        exists (proj1_sig f_i sup_X)...
+      - intros y.
+        split.
+        + intros H2 y' [ys [H3 H4]].
+          inversion H3; subst.
+          rename x into f_i.
+          assert (H6 := claim1 f_i H5).
+          assert (H7 : y' = proj1_sig f_i sup_X) by now apply (isSupremum_unique (image (fun x : D => proj1_sig f_i x) X)).
+          transitivity (proj1_sig f_i sup_X)...
+          apply claim2...
+          apply (in_image (fun f_i0 : D ~> D' => proj1_sig f_i0 sup_X))...
+        + intros H2.
+          apply claim2.
+          intros y' H3.
+          inversion H3; subst.
+          rename x into f_i.
+          apply H2.
+          exists (image (fun x : D => proj1_sig f_i x) X).
+          split...
+          apply (in_image (fun f_i0 : D ~> D' => image (fun x : D => proj1_sig f_i0 x) X))...
+    }
+    assert (claim4 : isSupremum (f sup_X) (unions (image (fun x : D => image (fun f_i : D ~> D' => proj1_sig f_i x) fs) X))).
+    { enough (H2 : forall x' : D', member x' (unions (image (fun f_i : D ~> D' => image (fun x : D => proj1_sig f_i x) X) fs)) <-> member x' (unions (image (fun x : D => image (fun f_i : D ~> D' => proj1_sig f_i x) fs) X))) by now apply (proj2 (isSupremum_ext _ _ H2 _ claim3 _) eq_refl).
+      intros y.
+      split.
+      - intros H2.
+        inversion H2; subst.
+        rename xs into ys.
+        inversion H4; subst.
+        rename x into f_i.
+        inversion H3; subst.
+        apply (in_unions (image (fun f_i' : D ~> D' => proj1_sig f_i' x) fs)).
+        + apply (in_image (fun f_i' : D ~> D' => proj1_sig f_i' x))...
+        + apply (in_image (fun x0 : D => image (fun f_i0 : D ~> D' => proj1_sig f_i0 x0) fs))...
+      - intros H2.
+        inversion H2; subst.
+        rename xs into ys.
+        inversion H4; subst.
+        inversion H3; subst.
+        rename x0 into f_i.
+        apply (in_unions (image (fun x' : D => proj1_sig f_i x') X)).
+        + apply (in_image (fun x' : D => proj1_sig f_i x'))...
+        + apply (in_image (fun f_i0 : D ~> D' => image (fun x0 : D => proj1_sig f_i0 x0) X))...
+    }
+    assert (claim5 : isSupremum (f sup_X) (image_sup (image (fun x : D => image (fun f_i : D ~> D' => proj1_sig f_i x) fs) X))).
+    { apply isSupremum_unions_Xs_iff_isSupremum_image_sup_Xs...
+      intros ys H2.
+      inversion H2; subst.
+      exists (f x).
+      intros y.
+      split.
+      - intros H4 y' H5.
+        inversion H5; subst.
+        rename x0 into f_i.
+        apply (proj2_sig (square_up_exists (image (fun f_i : D ~> D' => proj1_sig f_i x) fs) (sup_of_squigarrow_is_well_defined fs H x)))...
+      - intros H4.
+        assert (H5 : isSupremum (f x) (image (fun f_i : D ~> D' => proj1_sig f_i x) fs)) by apply (proj2_sig (square_up_exists (image (fun f_i : D ~> D' => proj1_sig f_i x) fs) (sup_of_squigarrow_is_well_defined fs H x))).
+        apply H5...
+    }
+    assert (claim6 : isSupremum (f sup_X) (image f X)).
+    { intros y.
+      split.
+      - intros H2 y' H3.
+        inversion H3; subst.
+        apply claim5...
+        exists (image (fun f_i : D ~> D' => proj1_sig f_i x) fs).
+        split.
+        + apply (in_image (fun x0 : D => image (fun f_i : D ~> D' => proj1_sig f_i x0) fs))...
+        + apply (proj2_sig (square_up_exists (image (fun f_i : D ~> D' => proj1_sig f_i x) fs) (sup_of_squigarrow_is_well_defined fs H x))).
+      - intros H2.
+        apply claim5.
+        intros y' [ys [H3 H4]].
+        inversion H3; subst.
+        assert (H6 : isSupremum (f x) (image (fun f_i : D ~> D' => proj1_sig f_i x) fs)) by apply (proj2_sig (square_up_exists (image (fun f_i : D ~> D' => proj1_sig f_i x) fs) (sup_of_squigarrow_is_well_defined fs H x))).
+        assert (H7 : y' = f x) by now apply (isSupremum_unique (image (fun f_i : D ~> D' => proj1_sig f_i x) fs)).
+        transitivity (f x)...
+    }
+    split...
+  Qed.
+
+  Local Program Instance squigarrow_isCompletePartialOrder {D : Type} {D' : Type} (D_requiresCompletePartialOrder : isCompletePartialOrder D) (D'_requiresCompletePartialOrder : isCompletePartialOrder D') : isCompletePartialOrder (D ~> D') :=
+    { CompletePartialOrder_requiresPoset := squigarrow_isPoset D_requiresCompletePartialOrder D'_requiresCompletePartialOrder
+    }
+  .
+
+  Next Obligation.
+    set (bot := fun _ : D => proj1_sig bottom_exists).
+    assert (claim1 : isContinuousMap bot).
+    { intros Y [H H0].
+      split.
+      - intros x1 x2 H1 H2.
+        inversion H1; subst.
+        apply (in_preimage bot).
+        apply (H (bot x1) (bot x2) H3 (Poset_refl (proj1_sig bottom_exists))).
+      - intros X [[x_0 H1] H2] sup_X H3 H4.
+        inversion H4; subst.
+        exists x_0.
+        constructor.
+        + apply H1.
+        + apply (in_preimage bot).
+          apply (H (bot sup_X) (bot x_0) H5).
+          apply Poset_refl.
+    }
+    exists (exist _ bot claim1).
+    simpl.
+    intros f x.
+    apply (proj2_sig bottom_exists).
+  Defined.
+
+  Next Obligation.
+    rename X into fs, H into fs_isDirected.
+    set (sup_fs := fun x : D => proj1_sig (square_up_exists (image (fun f_i : D ~> D' => proj1_sig f_i x) fs) (sup_of_squigarrow_is_well_defined fs fs_isDirected x))).
+    exists (exist _ sup_fs (sup_of_set_of_squigarrows_exists_if_it_is_directed fs fs_isDirected)).
+    assert (claim1 : forall x : D, isSupremum (sup_fs x) (image (fun f_i : D ~> D' => proj1_sig f_i x) fs)) by apply (fun x : D => proj2_sig (square_up_exists (image (fun f_i : D ~> D' => proj1_sig f_i x) fs) (sup_of_squigarrow_is_well_defined fs fs_isDirected x))).
+    intros f.
+    simpl.
+    split.
+    - intros H f' H0 x.
+      apply (claim1 x).
+      + apply H.
+      + apply (in_image (fun f_i : D ~> D' => proj1_sig f_i x)).  
+        apply H0.
+    - intros H x.
+      apply (claim1 x).
+      intros f' H0.
+      inversion H0; subst.
+      rename x0 into f'.
+      apply (H f').
+      apply H1.
+  Defined.
+
+  Lemma separately_continuous_iff {D1 : Type} {D2 : Type} {D3 : Type} `{D1_isCompletePartialOrder : isCompletePartialOrder D1} `{D2_isCompletePartialOrder : isCompletePartialOrder D2} `{D3_isCompletePartialOrder : isCompletePartialOrder D3} :
+    forall f : D1 * D2 -> D3,
+    ((forall x1 : D1, isContinuousMap (fun x2 : D2 => f (x1, x2))) /\ (forall x2 : D2, isContinuousMap (fun x1 : D1 => f (x1, x2)))) <-> isContinuousMap f.
+  Proof with eauto with *.
+    intros f.
+    split.
+    - intros [H H0].
+      apply the_main_reason_for_introducing_ScottTopology.
+      intros X H1 Y.
+      destruct (square_up_exists X H1) as [[sup_X1 sup_X2] H2].
+      set (X1 := getFsts X).
+      set (X2 := getSnds X).
+      exists (sup_X1, sup_X2), (f (sup_X1, sup_X2)).
+      assert (claim1 : isDirected X1).
+      { destruct H1 as [[[x1_0 x2_0] H1] H3].
+        split.
+        - exists x1_0.
+          apply (in_getFsts x1_0 x2_0)...
+        - intros x1_1 H4 x1_2 H5.
+          inversion H4; subst.
+          inversion H5; subst.
+          rename x' into x2_1, x'0 into x2_2.
+          destruct (H3 (x1_1, x2_1) H6 (x1_2, x2_2) H7) as [[x3_1 x3_2] [H8 [[H9 H10] [H11 H12]]]].
+          exists x3_1.
+          split...
+          apply (in_getFsts x3_1 x3_2)...
+      }
+      assert (claim2 : isDirected X2).
+      { destruct H1 as [[[x1_0 x2_0] H1] H3].
+        split.
+        - exists x2_0.
+          apply (in_getSnds x1_0 x2_0)...
+        - intros x2_1 H4 x2_2 H5.
+          inversion H4; subst.
+          inversion H5; subst.
+          rename x into x1_1, x0 into x1_2.
+          destruct (H3 (x1_1, x2_1) H6 (x1_2, x2_2) H7) as [[x3_1 x3_2] [H8 [[H9 H10] [H11 H12]]]].
+          exists x3_2.
+          split...
+          apply (in_getSnds x3_1 x3_2)...
+      }
+      assert ( claim3 :
+        forall x1 : D1,
+        exists sup_X2_x1 : D2, exists sup_f_X2_x1 : D3, isSupremum sup_X2_x1 X2 /\ isSupremum sup_f_X2_x1 (image (fun x2 : D2 => f (x1, x2)) X2) /\ f (x1, sup_X2_x1) = sup_f_X2_x1
+      ).
+      { intros x1.
+        apply (the_main_reason_for_introducing_ScottTopology (fun x2 : D2 => f (x1, x2)))...
+      }
+      assert ( claim4 :
+        forall x2 : D2,
+        exists sup_X1_x2 : D1, exists sup_f_X1_x2 : D3, isSupremum sup_X1_x2 X1 /\ isSupremum sup_f_X1_x2 (image (fun x1 : D1 => f (x1, x2)) X1) /\ f (sup_X1_x2, x2) = sup_f_X1_x2
+      ).
+      { intros x2.
+        apply (the_main_reason_for_introducing_ScottTopology (fun x1 : D1 => f (x1, x2)))...
+      }
+      assert (XXX : isSupremum sup_X1 X1 /\ isSupremum sup_X2 X2).
+      { destruct (square_up_exists X1 claim1) as [sup_X1' H3].
+        destruct (square_up_exists X2 claim2) as [sup_X2' H4].
+        assert (H5 : isSupremum (sup_X1', sup_X2') X).
+        { intros [x1 x2].
+          split.
+          - intros [H5 H6] [x1' x2'] H7.
+            simpl in *.
+            split.
+            + apply H3...
+              apply (in_getFsts x1' x2')...
+            + apply H4...
+              apply (in_getSnds x1' x2')...
+          - intros H5.
+            split.
+            + apply H3.
+              intros x1' H6.
+              inversion H6; subst.
+              rename x' into x2'.
+              apply (proj1 (H5 (x1', x2') H7)).
+            + apply H4.
+              intros x2' H6.
+              inversion H6; subst.
+              rename x into x1'.
+              apply (proj2 (H5 (x1', x2') H7)).
+          }
+        assert (H6 : (sup_X1, sup_X2) = (sup_X1', sup_X2')) by now apply (isSupremum_unique X).
+        inversion H6; subst.
+        simpl in *.
+        split...
+      }
+      destruct XXX as [claim5 claim6].
+      assert (claim7 : isSupremum (f (sup_X1, sup_X2)) (image (fun x2 : D2 => f (sup_X1, x2)) X2)).
+      { destruct (claim3 sup_X1) as [sup_X2_x1 [sup_f_X1_x2 [H3 [H4 H5]]]].
+        assert (H6 : isSupremum (f (sup_X1, sup_X2)) (image (fun x2 : D2 => f (sup_X1, x2)) X2) <-> sup_f_X1_x2 = f (sup_X1, sup_X2)) by now apply (@isSupremum_unique D3 (@CompletePartialOrder_requiresPoset D3 D3_isCompletePartialOrder)).
+        apply H6.
+        transitivity (f (sup_X1, sup_X2_x1)).
+        - symmetry...
+        - enough (H7 : sup_X2_x1 = sup_X2) by congruence.
+          apply (isSupremum_unique X2)...
+      }
+      assert ( claim8 :
+        forall x2 : D2,
+        member x2 X2 ->
+        isSupremum (f (sup_X1, x2)) (image (fun x1 : D1 => f (x1, x2)) X1)
+      ).
+      { intros x2 H3.
+        destruct (claim4 x2) as [sup_X1' [sup_f_X1_x2' [H4 [H5 H6]]]].
+        assert (H7 : isSupremum (f (sup_X1, x2)) (image (fun x1 : D1 => f (x1, x2)) X1) <-> sup_f_X1_x2' = f (sup_X1, x2)) by now apply (@isSupremum_unique D3 (@CompletePartialOrder_requiresPoset D3 D3_isCompletePartialOrder)).
+        apply H7.
+        transitivity (f (sup_X1', x2)).
+        - symmetry...
+        - enough (H8 : sup_X1' = sup_X1) by congruence.
+          apply (isSupremum_unique X1)...
+      }
+      assert (claim9 : isSupremum (f (sup_X1, sup_X2)) (image_sup (image (fun x2 : D2 => image (fun x1 : D1 => f (x1, x2)) X1) X2))).
+      { intros y.
+        split.
+        - intros H3 y' [ys [H4 H5]].
+          inversion H4; subst.
+          rename x into x2.
+          assert (H7 : isSupremum (f (sup_X1, x2)) (image (fun x1 : D1 => f (x1, x2)) X1)) by now apply claim8.
+          assert (H8 : y' = (f (sup_X1, x2))) by now apply (isSupremum_unique (image (fun x1 : D1 => f (x1, x2)) X1)).
+          assert (H9 : f (sup_X1, x2) =< f (sup_X1, sup_X2)).
+          { apply (ContinuousMaps_on_cpos_are_always_monotonic (fun x2' : D2 => f (sup_X1, x2')) (H sup_X1)).
+            apply claim6...
+          }
+          transitivity (f (sup_X1, x2))...
+        - intros H7.
+          apply claim7.
+          intros y' H8.
+          inversion H8; subst.
+          rename x into x2.
+          apply H7...
+          exists (image (fun x1 : D1 => f (x1, x2)) X1).
+          split.
+          + apply (in_image (fun x0 : D2 => image (fun x1 : D1 => f (x1, x0)) X1))...
+          + apply claim8...
+      }
+      assert (claim10 : isSupremum (f (sup_X1, sup_X2)) (unions (image (fun x2 : D2 => image (fun x1 : D1 => f (x1, x2)) X1) X2))).
+      { apply isSupremum_unions_Xs_iff_isSupremum_image_sup_Xs...
+        intros ys H3.
+        inversion H3; subst.
+        rename x into x2.
+        exists (f (sup_X1, x2))...
+      }
+      assert (claim11 : isSupremum (f (sup_X1, sup_X2)) (image f X)).
+      { intros y.
+        split.
+        - intros H3 y' H4.
+          inversion H4; subst.
+          apply claim10.
+          + apply H3.
+          + destruct x as [x1 x2].
+            apply (in_unions (image (fun x1' : D1 => f (x1', x2)) X1)).
+            * apply (in_image (fun x1' : D1 => f (x1', x2))).
+              apply (in_getFsts x1 x2)...
+            * apply (in_image (fun x0 : D2 => image (fun x3 : D1 => f (x3, x0)) X1)).
+              apply (in_getSnds x1 x2)...
+        - intros H3.
+          apply claim10.
+          intros y' H4.
+          inversion H4; subst.
+          rename xs into ys.
+          inversion H6; subst.
+          rename x into x2_2.
+          inversion H5; subst.
+          rename x into x1_1.
+          inversion H8; subst.
+          rename x' into x2_1.
+          inversion H7; subst.
+          rename x into x1_2.
+          destruct H1 as [H1 H11].
+          destruct (H11 (x1_1, x2_1) H9 (x1_2, x2_2) H10) as [[x3_1 x3_2] [H12 [[H13 H14] [H15 H16]]]].
+          simpl in *.
+          assert (H17 : f (x1_1, x2_2) =< f (x3_1, x3_2)).
+          { transitivity (f (x1_1, x3_2)).
+            - apply (ContinuousMaps_on_cpos_are_always_monotonic (fun x2 : D2 => f (x1_1, x2)))...
+            - apply (ContinuousMaps_on_cpos_are_always_monotonic (fun x1 : D1 => f (x1, x3_2)))...
+          }
+          transitivity (f (x3_1, x3_2))...
+      }
+      split...
+    - intros H.
+      split.
+      + intros x1.
+        apply (the_main_reason_for_introducing_ScottTopology (fun x2 : D2 => f (x1, x2))).
+        intros X2 H0 Y.
+        destruct (square_up_exists X2 H0) as [sup_X2 H1].
+        set (X := image (fun x2 : D2 => (x1, x2)) X2).
+        assert (claim1 : isDirected X).
+        { destruct H0 as [[x2_0 H0] H2].
+          split.
+          - exists (x1, x2_0).
+            apply (in_image (fun x2 : D2 => (x1, x2)))...
+          - intros [x1_1 x2_1] H3 [x1_2 x2_2] H4.
+            inversion H3; subst x1_1; subst.
+            inversion H4; subst x1_2; subst.
+            rename H8 into H5, H9 into H6.
+            destruct (H2 x2_1 H5 x2_2 H6) as [x3_2 [H7 [H8 H9]]].
+            exists (x1, x3_2).
+            repeat split...
+        }
+        destruct (square_up_exists X claim1) as [sup_X H2].
+        exists sup_X2, (f sup_X).
+        assert (claim2 : (x1, sup_X2) = sup_X).
+        { apply (isSupremum_unique X)...
+          intros [x_1 x_2].
+          split.
+          - intros [H3 H4] [x_1' x_2'] H5.
+            inversion H5; subst x_1'; subst.
+            simpl.
+            split...
+          - intros H3.
+            simpl.
+            split.
+            + destruct H0 as [[x2_0 H0] H4].
+              apply (H3 (x1, x2_0))...
+            + apply H1.
+              intros x_2' H4.
+              apply (H3 (x1, x_2'))...
+        }
+        assert (claim3 : f (x1, sup_X2) = f sup_X) by congruence.
+        assert (XXX : exists sup_X' : D1 * D2, exists sup_Y' : D3, isSupremum sup_X' X /\ isSupremum sup_Y' (image f X) /\ f sup_X' = sup_Y') by now apply the_main_reason_for_introducing_ScottTopology.
+        destruct XXX as [sup_X' [sup_Y' [H3 [H4 H5]]]].
+        assert (claim4 : isSupremum (f sup_X) Y).
+        { assert (H6 : isSupremum (f sup_X) (image f X) <-> sup_Y' = f sup_X) by now apply (@isSupremum_unique D3 (@CompletePartialOrder_requiresPoset D3 D3_isCompletePartialOrder) (image f X)).
+          assert (H7 : isSupremum (f sup_X) (image f X)).
+          { apply H6.
+            transitivity (f sup_X').
+            - symmetry...
+            - enough (H7 : sup_X' = sup_X) by congruence.
+              apply (isSupremum_unique X)...
+          }
+          assert (H8 : forall y : D3, member y (image f X) <-> member y Y).
+          { intros y.
+            split.
+            - intros H8.
+              inversion H8; subst.
+              inversion H9; subst.
+              rename x0 into x2.
+              apply (in_image (fun x2 : D2 => f (x1, x2)))...
+            - intros H8.
+              inversion H8; subst.
+              rename x into x2.
+              apply (in_image f)...
+          }
+          apply (proj2 (@isSupremum_ext D3 (@CompletePartialOrder_requiresPoset D3 D3_isCompletePartialOrder) _ _ H8 _ H7 _) eq_refl).
+        }
+        split...
+      + intros x2.
+        apply (the_main_reason_for_introducing_ScottTopology (fun x1 : D1 => f (x1, x2))).
+        intros X1 H0 Y.
+        destruct (square_up_exists X1 H0) as [sup_X1 H1].
+        set (X := image (fun x1 : D1 => (x1, x2)) X1).
+        assert (YYY : forall x1 : D1, member x1 X1 -> member (x1, x2) X).
+        { intros x1 H2.
+          apply (in_image (fun x1 : D1 => (x1, x2))), H2.
+        }
+        assert (claim1 : isDirected X).
+        { destruct H0 as [[x1_0 H0] H2].
+          split.
+          - exists (x1_0, x2).
+            apply (in_image (fun x1 : D1 => (x1, x2)))...
+          - intros [x1_1 x2_1] H3 [x1_2 x2_2] H4.
+            inversion H3; subst x2_1; subst.
+            inversion H4; subst x2_2; subst.
+            rename H8 into H5, H9 into H6.
+            destruct (H2 x1_1 H5 x1_2 H6) as [x3_1 [H7 [H8 H9]]].
+            exists (x3_1, x2).
+            repeat split...
+        }
+        destruct (square_up_exists X claim1) as [sup_X H2].
+        exists sup_X1, (f sup_X).
+        assert (claim2 : (sup_X1, x2) = sup_X).
+        { apply (isSupremum_unique X)...
+          intros [x_1 x_2].
+          split.
+          - intros [H3 H4] [x_1' x_2'] H5.
+            inversion H5; subst x_1'; subst.
+            simpl.
+            split...
+          - intros H3.
+            simpl.
+            split.
+            + apply H1.
+              intros x_1' H4.
+              apply (H3 (x_1', x2))...
+            + destruct H0 as [[x1_0 H0] H4].
+              apply (H3 (x1_0, x2))...
+        }
+        assert (claim3 : f (sup_X1, x2) = f sup_X) by congruence.
+        assert (XXX : exists sup_X' : D1 * D2, exists sup_Y' : D3, isSupremum sup_X' X /\ isSupremum sup_Y' (image f X) /\ f sup_X' = sup_Y') by now apply the_main_reason_for_introducing_ScottTopology.
+        destruct XXX as [sup_X' [sup_Y' [H3 [H4 H5]]]].
+        assert (claim4 : isSupremum (f sup_X) Y).
+        { assert (H6 : isSupremum (f sup_X) (image f X) <-> sup_Y' = f sup_X) by now apply (@isSupremum_unique D3 (@CompletePartialOrder_requiresPoset D3 D3_isCompletePartialOrder) (image f X)).
+          assert (H7 : isSupremum (f sup_X) (image f X)).
+          { apply H6.
+            transitivity (f sup_X').
+            - symmetry...
+            - enough (H7 : sup_X' = sup_X) by congruence.
+              apply (isSupremum_unique X)...
+          }
+          assert (H8 : forall y : D3, member y (image f X) <-> member y Y).
+          { intros y.
+            split.
+            - intros H8.
+              inversion H8; subst.
+              inversion H9; subst.
+              rename x0 into x1.
+              apply (in_image (fun x1 : D1 => f (x1, x2)))...
+            - intros H8.
+              inversion H8; subst.
+              rename x into x1.
+              apply (in_image f)...
+          }
+          apply (proj2 (@isSupremum_ext D3 (@CompletePartialOrder_requiresPoset D3 D3_isCompletePartialOrder) _ _ H8 _ H7 _) eq_refl).
+        }
+        split...
+  Qed.
+
+End DomainTheory.
+
+Module UntypedLamdbdaCalculus.
+
+  Import ListNotations.
+
+  Import MyUtilities.
+
+  Import MyStructures.
+
+  Import MyEnsemble.
+
+  Import GeneralTopology.
+
+  Import DomainTheory.
+
+  Definition ivar : Set :=
+    nat
+  .
+
+  Definition ivar_eq_dec :
+    forall x : ivar,
+    forall y : ivar,
+    {x = y} + {x <> y}.
+  Proof.
+    apply Nat.eq_dec.
+  Defined.
+
+  Inductive tm : Set :=
+  | tmVar : forall x : ivar, tm
+  | tmApp : forall P1 : tm, forall P2 : tm, tm
+  | tmLam : forall y : ivar, forall Q : tm, tm
+  .
+
+  Definition tm_eq_dec :
+    forall M1 : tm,
+    forall M2 : tm,
+    {M1 = M2} + {M1 <> M2}.
+  Proof with try ((left; congruence) || (right; congruence)).
+    induction M1; destruct M2...
+    - destruct (ivar_eq_dec x x0)...
+    - destruct (IHM1_1 M2_1); destruct (IHM1_2 M2_2)...
+    - destruct (ivar_eq_dec y y0); destruct (IHM1 M2)...
+  Defined.
+
+  Fixpoint getRank (M : tm) {struct M} : nat :=
+    match M with
+    | tmVar x => 0
+    | tmApp P1 P2 => S (max (getRank P1) (getRank P2))
+    | tmLam y Q => S (getRank Q)
+    end
+  .
+
+  Inductive subtm : tm -> tm -> Set :=
+  | subtmRefl : forall M : tm, subtm M M
+  | subtmAppL : forall M : tm, forall P1 : tm, forall P2 : tm, subtm M P1 -> subtm M (tmApp P1 P2)
+  | subtmAppR : forall M : tm, forall P1 : tm, forall P2 : tm, subtm M P2 -> subtm M (tmApp P1 P2)
+  | subtmLAbs : forall M : tm, forall y : ivar, forall Q : tm, subtm M Q -> subtm M (tmLam y Q)
+  .
+
+  Global Hint Constructors tm : my_hints.
+
+  Lemma subtm_getRank :
     forall M : tm,
-    forall X : subtm N M,
-    forall H : N = tmVar z,
-    XP z M (eq_rect N (fun N0 : tm => subtm N0 M) X (tmVar z) H)
-  ).
-  { assert ( XP_Refl :
-      forall M0 : tm,
-      forall H : M0 = tmVar z,
-      XP z M0 (eq_rect M0 (fun N1 : tm => subtm N1 M0) (subtmRefl M0) (tmVar z) H)
+    forall N : tm,
+    subtm M N ->
+    getRank M <= getRank N.
+  Proof with lia.
+    intros M N X.
+    induction X; simpl...
+  Qed.
+
+  Lemma subtm_and_same_rank_implies_same_term :
+    forall M : tm,
+    forall N : tm,
+    subtm M N ->
+    getRank M = getRank N ->
+    M = N.
+  Proof with lia.
+    intros M N X.
+    destruct X; intros.
+    - reflexivity.
+    - assert (H0 := subtm_getRank M P1 X).
+      simpl in *...
+    - assert (H0 := subtm_getRank M P2 X).
+      simpl in *...
+    - assert (H0 := subtm_getRank M Q X).
+      simpl in *...
+  Qed.
+
+  Lemma subtm_refl :
+    forall M1 : tm,
+    subtm M1 M1.
+  Proof.
+    apply subtmRefl.
+  Qed.
+
+  Local Hint Resolve subtm_refl : core.
+
+  Lemma subtm_asym :
+    forall M1 : tm,
+    forall M2 : tm,
+    subtm M1 M2 ->
+    subtm M2 M1 ->
+    M1 = M2.
+  Proof with eauto.
+    intros.
+    apply subtm_and_same_rank_implies_same_term...
+    enough (getRank M1 <= getRank M2 /\ getRank M2 <= getRank M1) by lia.
+    split; apply subtm_getRank...
+  Qed.
+
+  Local Hint Resolve subtm_asym : core.
+
+  Lemma subtm_trans :
+    forall M1 : tm,
+    forall M2 : tm,
+    forall M3 : tm,
+    subtm M1 M2 ->
+    subtm M2 M3 ->
+    subtm M1 M3.
+  Proof with eauto.
+    enough (claim1 : forall L : tm, forall N : tm, forall M : tm, subtm N L -> subtm M N -> subtm M L)...
+    induction L.
+    all: intros; inversion H; subst...
+    - constructor 2...
+    - constructor 3...
+    - constructor 4...
+  Qed.
+
+  Local Hint Resolve subtm_trans : core.
+
+  Theorem strong_induction_on_tm (phi : tm -> Prop) :
+    (forall M : tm, (forall N : tm, subtm N M -> N <> M -> phi N) -> phi M) ->
+    forall M : tm,
+    phi M.
+  Proof with try now (firstorder; eauto).
+    intros XXX.
+    enough (claim1 : forall M : tm, forall L : tm, subtm L M -> phi L)...
+    induction M.
+    all: intros L H; apply XXX; intros N H0 H1; inversion H0; subst...
+    all: inversion H; subst...
+  Qed.
+
+  Definition occurence_rect (XP : forall z : ivar, forall M : tm, subtm (tmVar z) M -> Type) :
+    (forall x : ivar, XP x (tmVar x) (subtmRefl (tmVar x))) ->
+    (forall x : ivar, forall P1 : tm, forall P2 : tm, forall X : subtm (tmVar x) P1, XP x P1 X -> XP x (tmApp P1 P2) (subtmAppL (tmVar x) P1 P2 X)) ->
+    (forall x : ivar, forall P1 : tm, forall P2 : tm, forall X : subtm (tmVar x) P2, XP x P2 X -> XP x (tmApp P1 P2) (subtmAppR (tmVar x) P1 P2 X)) ->
+    (forall x : ivar, forall y : ivar, forall Q : tm, forall X : subtm (tmVar x) Q, XP x Q X -> XP x (tmLam y Q) (subtmLAbs (tmVar x) y Q X)) ->
+    (forall x : ivar, forall M : tm, forall X : subtm (tmVar x) M, XP x M X).
+  Proof.
+    intros XP_refl XP_appl XP_appr XP_labs z.
+    assert ( XXX :
+      forall N : tm,
+      forall M : tm,
+      forall X : subtm N M,
+      forall H : N = tmVar z,
+      XP z M (eq_rect N (fun N0 : tm => subtm N0 M) X (tmVar z) H)
     ).
-    { intros M0.
-      apply (case_eq M0 (tmVar z) (fun M1 : tm => fun H0 : M1 = tmVar z => XP z M1 (eq_rect M1 (fun N1 : tm => subtm N1 M1) (subtmRefl M1) (tmVar z) H0))).
-      apply (XP_refl z).
-    }
-    assert ( XP_AppL :
-      forall M0 : tm,
-      forall P1 : tm,
-      forall P2 : tm,
-      forall H : M0 = tmVar z,
-      forall X' : subtm M0 P1,
-      (forall H' : M0 = tmVar z, XP z P1 (eq_rect M0 (fun N1 : tm => subtm N1 P1) X' (tmVar z) H')) ->
-      XP z (tmApp P1 P2) (eq_rect M0 (fun N1 : tm => subtm N1 (tmApp P1 P2)) (subtmAppL M0 P1 P2 X') (tmVar z) H)
-    ).
-    { intros M0 P1 P2.
-      apply (case_eq M0 (tmVar z) (fun M1 : tm => fun H0 : M1 = tmVar z => forall X' : subtm M1 P1, (forall H' : M1 = tmVar z, XP z P1 (eq_rect M1 (fun N1 : tm => subtm N1 P1) X' (tmVar z) H')) -> XP z (tmApp P1 P2) (eq_rect M1 (fun N1 : tm => subtm N1 (tmApp P1 P2)) (subtmAppL M1 P1 P2 X') (tmVar z) H0))).
-      apply (fun X' : subtm (tmVar z) P1 => fun IHX' : forall H' : tmVar z = tmVar z, XP z P1 (eq_rect (tmVar z) (fun N1 : tm => subtm N1 P1) X' (tmVar z) H') => XP_appl z P1 P2 X' (IHX' eq_refl)).
-    }
-    assert ( XP_AppR :
-      forall M0 : tm,
-      forall P1 : tm,
-      forall P2 : tm,
-      forall H : M0 = tmVar z,
-      forall X' : subtm M0 P2,
-      (forall H' : M0 = tmVar z, XP z P2 (eq_rect M0 (fun N1 : tm => subtm N1 P2) X' (tmVar z) H')) ->
-      XP z (tmApp P1 P2) (eq_rect M0 (fun N1 : tm => subtm N1 (tmApp P1 P2)) (subtmAppR M0 P1 P2 X') (tmVar z) H)
-    ).
-    { intros M0 P1 P2.
-      apply (case_eq M0 (tmVar z) (fun M1 : tm => fun H0 : M1 = tmVar z => forall X' : subtm M1 P2, (forall H' : M1 = tmVar z, XP z P2 (eq_rect M1 (fun N1 : tm => subtm N1 P2) X' (tmVar z) H')) -> XP z (tmApp P1 P2) (eq_rect M1 (fun N1 : tm => subtm N1 (tmApp P1 P2)) (subtmAppR M1 P1 P2 X') (tmVar z) H0))).
-      apply (fun X' : subtm (tmVar z) P2 => fun IHX' : forall H' : tmVar z = tmVar z, XP z P2 (eq_rect (tmVar z) (fun N1 : tm => subtm N1 P2) X' (tmVar z) H') => XP_appr z P1 P2 X' (IHX' eq_refl)).
-    }
-    assert ( XP_LAbs :
-      forall M0 : tm,
-      forall y : ivar,
-      forall Q : tm,
-      forall H : M0 = tmVar z,
-      forall X' : subtm M0 Q,
-      (forall H' : M0 = tmVar z, XP z Q (eq_rect M0 (fun N1 : tm => subtm N1 Q) X' (tmVar z) H')) ->
-      XP z (tmLam y Q) (eq_rect M0 (fun N1 : tm => subtm N1 (tmLam y Q)) (subtmLAbs M0 y Q X') (tmVar z) H)
-    ).
-    { intros M0 y Q.
-      apply (case_eq M0 (tmVar z) (fun M1 : tm => fun H0 : M1 = tmVar z => forall X' : subtm M1 Q, (forall H' : M1 = tmVar z, XP z Q (eq_rect M1 (fun N1 : tm => subtm N1 Q) X' (tmVar z) H')) -> XP z (tmLam y Q) (eq_rect M1 (fun N1 : tm => subtm N1 (tmLam y Q)) (subtmLAbs M1 y Q X') (tmVar z) H0))).
-      apply (fun X' : subtm (tmVar z) Q => fun IHX' : forall H' : tmVar z = tmVar z, XP z Q (eq_rect (tmVar z) (fun N1 : tm => subtm N1 Q) X' (tmVar z) H') => XP_labs z y Q X' (IHX' eq_refl)).
+    { assert ( XP_Refl :
+        forall M0 : tm,
+        forall H : M0 = tmVar z,
+        XP z M0 (eq_rect M0 (fun N1 : tm => subtm N1 M0) (subtmRefl M0) (tmVar z) H)
+      ).
+      { intros M0.
+        apply (case_eq M0 (tmVar z) (fun M1 : tm => fun H0 : M1 = tmVar z => XP z M1 (eq_rect M1 (fun N1 : tm => subtm N1 M1) (subtmRefl M1) (tmVar z) H0))).
+        apply (XP_refl z).
+      }
+      assert ( XP_AppL :
+        forall M0 : tm,
+        forall P1 : tm,
+        forall P2 : tm,
+        forall H : M0 = tmVar z,
+        forall X' : subtm M0 P1,
+        (forall H' : M0 = tmVar z, XP z P1 (eq_rect M0 (fun N1 : tm => subtm N1 P1) X' (tmVar z) H')) ->
+        XP z (tmApp P1 P2) (eq_rect M0 (fun N1 : tm => subtm N1 (tmApp P1 P2)) (subtmAppL M0 P1 P2 X') (tmVar z) H)
+      ).
+      { intros M0 P1 P2.
+        apply (case_eq M0 (tmVar z) (fun M1 : tm => fun H0 : M1 = tmVar z => forall X' : subtm M1 P1, (forall H' : M1 = tmVar z, XP z P1 (eq_rect M1 (fun N1 : tm => subtm N1 P1) X' (tmVar z) H')) -> XP z (tmApp P1 P2) (eq_rect M1 (fun N1 : tm => subtm N1 (tmApp P1 P2)) (subtmAppL M1 P1 P2 X') (tmVar z) H0))).
+        apply (fun X' : subtm (tmVar z) P1 => fun IHX' : forall H' : tmVar z = tmVar z, XP z P1 (eq_rect (tmVar z) (fun N1 : tm => subtm N1 P1) X' (tmVar z) H') => XP_appl z P1 P2 X' (IHX' eq_refl)).
+      }
+      assert ( XP_AppR :
+        forall M0 : tm,
+        forall P1 : tm,
+        forall P2 : tm,
+        forall H : M0 = tmVar z,
+        forall X' : subtm M0 P2,
+        (forall H' : M0 = tmVar z, XP z P2 (eq_rect M0 (fun N1 : tm => subtm N1 P2) X' (tmVar z) H')) ->
+        XP z (tmApp P1 P2) (eq_rect M0 (fun N1 : tm => subtm N1 (tmApp P1 P2)) (subtmAppR M0 P1 P2 X') (tmVar z) H)
+      ).
+      { intros M0 P1 P2.
+        apply (case_eq M0 (tmVar z) (fun M1 : tm => fun H0 : M1 = tmVar z => forall X' : subtm M1 P2, (forall H' : M1 = tmVar z, XP z P2 (eq_rect M1 (fun N1 : tm => subtm N1 P2) X' (tmVar z) H')) -> XP z (tmApp P1 P2) (eq_rect M1 (fun N1 : tm => subtm N1 (tmApp P1 P2)) (subtmAppR M1 P1 P2 X') (tmVar z) H0))).
+        apply (fun X' : subtm (tmVar z) P2 => fun IHX' : forall H' : tmVar z = tmVar z, XP z P2 (eq_rect (tmVar z) (fun N1 : tm => subtm N1 P2) X' (tmVar z) H') => XP_appr z P1 P2 X' (IHX' eq_refl)).
+      }
+      assert ( XP_LAbs :
+        forall M0 : tm,
+        forall y : ivar,
+        forall Q : tm,
+        forall H : M0 = tmVar z,
+        forall X' : subtm M0 Q,
+        (forall H' : M0 = tmVar z, XP z Q (eq_rect M0 (fun N1 : tm => subtm N1 Q) X' (tmVar z) H')) ->
+        XP z (tmLam y Q) (eq_rect M0 (fun N1 : tm => subtm N1 (tmLam y Q)) (subtmLAbs M0 y Q X') (tmVar z) H)
+      ).
+      { intros M0 y Q.
+        apply (case_eq M0 (tmVar z) (fun M1 : tm => fun H0 : M1 = tmVar z => forall X' : subtm M1 Q, (forall H' : M1 = tmVar z, XP z Q (eq_rect M1 (fun N1 : tm => subtm N1 Q) X' (tmVar z) H')) -> XP z (tmLam y Q) (eq_rect M1 (fun N1 : tm => subtm N1 (tmLam y Q)) (subtmLAbs M1 y Q X') (tmVar z) H0))).
+        apply (fun X' : subtm (tmVar z) Q => fun IHX' : forall H' : tmVar z = tmVar z, XP z Q (eq_rect (tmVar z) (fun N1 : tm => subtm N1 Q) X' (tmVar z) H') => XP_labs z y Q X' (IHX' eq_refl)).
+      }
+      apply (
+        fix occurence_rect_fix (N : tm) (M : tm) (X : subtm N M) {struct X} : forall H : N = tmVar z, XP z M (eq_rect N (fun N1 : tm => subtm N1 M) X (tmVar z) H) :=
+        match X as X0 in subtm N0 M0 return forall H : N0 = tmVar z, XP z M0 (eq_rect N0 (fun N1 : tm => subtm N1 M0) X0 (tmVar z) H) with
+        | subtmRefl M0 =>
+          fun H : M0 = tmVar z =>
+          XP_Refl M0 H 
+        | subtmAppL M0 P1 P2 X' =>
+          fun H : M0 = tmVar z =>
+          XP_AppL M0 P1 P2 H X' (occurence_rect_fix M0 P1 X')
+        | subtmAppR M0 P1 P2 X' =>
+          fun H : M0 = tmVar z =>
+          XP_AppR M0 P1 P2 H X' (occurence_rect_fix M0 P2 X')
+        | subtmLAbs M0 y Q X' =>
+          fun H : M0 = tmVar z =>
+          XP_LAbs M0 y Q H X' (occurence_rect_fix M0 Q X')
+        end
+      ).
     }
     apply (
-      fix occurence_rect_fix (N : tm) (M : tm) (X : subtm N M) {struct X} : forall H : N = tmVar z, XP z M (eq_rect N (fun N1 : tm => subtm N1 M) X (tmVar z) H) :=
-      match X as X0 in subtm N0 M0 return forall H : N0 = tmVar z, XP z M0 (eq_rect N0 (fun N1 : tm => subtm N1 M0) X0 (tmVar z) H) with
-      | subtmRefl M0 =>
-        fun H : M0 = tmVar z =>
-        XP_Refl M0 H 
-      | subtmAppL M0 P1 P2 X' =>
-        fun H : M0 = tmVar z =>
-        XP_AppL M0 P1 P2 H X' (occurence_rect_fix M0 P1 X')
-      | subtmAppR M0 P1 P2 X' =>
-        fun H : M0 = tmVar z =>
-        XP_AppR M0 P1 P2 H X' (occurence_rect_fix M0 P2 X')
-      | subtmLAbs M0 y Q X' =>
-        fun H : M0 = tmVar z =>
-        XP_LAbs M0 y Q H X' (occurence_rect_fix M0 Q X')
-      end
+      fun M : tm =>
+      fun X : subtm (tmVar z) M =>
+      XXX (tmVar z) M X eq_refl
     ).
-  }
-  apply (
-    fun M : tm =>
-    fun X : subtm (tmVar z) M =>
-    XXX (tmVar z) M X eq_refl
-  ).
-Defined.
+  Defined.
 
-Fixpoint getFVs (M : tm) : list ivar :=
-  match M with
-  | tmVar x => [x]
-  | tmApp P1 P2 => getFVs P1 ++ getFVs P2
-  | tmLam y Q => remove ivar_eq_dec y (getFVs Q)
-  end
-.
+  Fixpoint getFVs (M : tm) : list ivar :=
+    match M with
+    | tmVar x => [x]
+    | tmApp P1 P2 => getFVs P1 ++ getFVs P2
+    | tmLam y Q => remove ivar_eq_dec y (getFVs Q)
+    end
+  .
 
-Fixpoint isFreeIn (z : ivar) (M : tm) {struct M} : bool :=
-  match M with
-  | tmVar x => Nat.eqb x z
-  | tmApp P1 P2 => isFreeIn z P1 || isFreeIn z P2
-  | tmLam y Q => isFreeIn z Q && negb (Nat.eqb z y)
-  end
-.
+  Fixpoint isFreeIn (z : ivar) (M : tm) {struct M} : bool :=
+    match M with
+    | tmVar x => Nat.eqb x z
+    | tmApp P1 P2 => isFreeIn z P1 || isFreeIn z P2
+    | tmLam y Q => isFreeIn z Q && negb (Nat.eqb z y)
+    end
+  .
 
-Lemma getFVs_isFreeIn (M : tm) :
-  forall z : ivar,
-  In z (getFVs M) <-> isFreeIn z M = true.
-Proof with try now firstorder.
-  induction M; simpl; intros z.
-  - rewrite Nat.eqb_eq...
-  - rewrite orb_true_iff, in_app_iff...
-  - rewrite andb_true_iff, negb_true_iff, Nat.eqb_neq.
-    split; intros H.
-    + apply in_remove in H...
-    + apply in_in_remove...
-Qed.
+  Lemma getFVs_isFreeIn (M : tm) :
+    forall z : ivar,
+    In z (getFVs M) <-> isFreeIn z M = true.
+  Proof with try now firstorder.
+    induction M; simpl; intros z.
+    - rewrite Nat.eqb_eq...
+    - rewrite orb_true_iff, in_app_iff...
+    - rewrite andb_true_iff, negb_true_iff, Nat.eqb_neq.
+      split; intros H.
+      + apply in_remove in H...
+      + apply in_in_remove...
+  Qed.
 
-End Occurences.
+  Definition substitution : Set :=
+    ivar -> tm
+  .
 
-Section Substitution.
+  Definition nil_subtitution : substitution :=
+    tmVar
+  .
 
-Definition substitution : Set :=
-  ivar -> tm
-.
+  Definition cons_substitution : ivar -> tm -> substitution -> substitution :=
+    fun x : ivar => fun M : tm => fun sigma : substitution => fun y : ivar => if ivar_eq_dec x y then M else sigma y
+  .
 
-Definition nil_subtitution : substitution :=
-  tmVar
-.
+  Fixpoint mk_substitution (sigma : list (ivar * tm)) {struct sigma} : substitution :=
+    match sigma with
+    | [] => nil_subtitution
+    | (x, M) :: sigma' => cons_substitution x M (mk_substitution sigma')
+    end
+  .
 
-Definition cons_substitution : ivar -> tm -> substitution -> substitution :=
-  fun x : ivar => fun M : tm => fun sigma : substitution => fun y : ivar => if ivar_eq_dec x y then M else sigma y
-.
+  Definition get_max_ivar : tm -> ivar :=
+    fun M : tm => fold_right_max_0 (getFVs M)
+  .
 
-Fixpoint mk_substitution (sigma : list (ivar * tm)) {struct sigma} : substitution :=
-  match sigma with
-  | [] => nil_subtitution
-  | (x, M) :: sigma' => cons_substitution x M (mk_substitution sigma')
-  end
-.
-
-Definition get_max_ivar : tm -> ivar :=
-  fun M : tm => fold_right_max_0 (getFVs M)
-.
-
-Lemma get_max_ivar_lt (M : tm) :
-  forall x : ivar,
-  get_max_ivar M < x ->
-  isFreeIn x M = false.
-Proof with lia.
-  intros x.
-  enough (get_max_ivar M < x -> ~ In x (getFVs M)) by now rewrite getFVs_isFreeIn, not_true_iff_false in H.
-  assert (H1 : In x (getFVs M) -> fold_right_max_0 (getFVs M) >= x) by apply fold_right_max_0_in.
-  enough (fold_right_max_0 (getFVs M) >= x -> fold_right_max_0 (getFVs M) < x -> False) by now eauto...
-Qed.
-
-Definition isFreshIn_substitution : ivar -> substitution -> tm -> bool :=
-  fun x : ivar => fun sigma : substitution => fun M : tm => forallb (fun z : ivar => negb (isFreeIn x (sigma z))) (getFVs M)
-.
-
-Definition chi : substitution -> tm -> ivar :=
-  fun sigma : substitution => fun M : tm => S (fold_right_max_0 (map (fun x : ivar => get_max_ivar (sigma x)) (getFVs M)))
-.
-
-Theorem main_property_of_chi :
-  forall M : tm,
-  forall sigma : substitution,
-  isFreshIn_substitution (chi sigma M) sigma M = true.
-Proof with try now firstorder.
-  assert ( claim1 :
-    forall sigma : substitution,
-    forall M : tm,
+  Lemma get_max_ivar_lt (M : tm) :
     forall x : ivar,
-    isFreeIn x M = true ->
-    isFreeIn (chi sigma M) (sigma x) = false
-  ).
-  { intros sigma M x H.
-    enough (get_max_ivar (sigma x) < chi sigma M) by now apply get_max_ivar_lt.
-    unfold chi, fold_right_max_0.
-    enough (fold_right max 0 (map (fun z : ivar => get_max_ivar (sigma z)) (getFVs M)) >= get_max_ivar (sigma x)) by lia.
-    rewrite <- getFVs_isFreeIn in H.
-    apply fold_right_max_0_in, in_map_iff...
-  }
-  unfold isFreshIn_substitution.
-  intros M sigma.
-  apply forallb_true_iff.
-  intros x H.
-  apply negb_true_iff, claim1, getFVs_isFreeIn...
-Qed.
+    get_max_ivar M < x ->
+    isFreeIn x M = false.
+  Proof with lia.
+    intros x.
+    enough (get_max_ivar M < x -> ~ In x (getFVs M)) by now rewrite getFVs_isFreeIn, not_true_iff_false in H.
+    assert (H1 : In x (getFVs M) -> fold_right_max_0 (getFVs M) >= x) by apply fold_right_max_0_in.
+    enough (fold_right_max_0 (getFVs M) >= x -> fold_right_max_0 (getFVs M) < x -> False) by now eauto...
+  Qed.
 
-Lemma chi_nil : 
-  forall M : tm,
-  isFreeIn (chi nil_subtitution M) M = false.
-Proof with try now firstorder.
-  intros M.
-  assert (H : isFreshIn_substitution (chi nil_subtitution M) nil_subtitution M = true) by apply main_property_of_chi.
-  unfold isFreshIn_substitution in H.
-  rewrite forallb_true_iff in H.
-  simpl in H.
-  apply not_true_iff_false.
-  intros H0.
-  assert (H1 : negb (chi nil_subtitution M =? chi nil_subtitution M) = true) by now apply H, getFVs_isFreeIn.
-  rewrite negb_true_iff, Nat.eqb_neq in H1...
-Qed.
+  Definition isFreshIn_substitution : ivar -> substitution -> tm -> bool :=
+    fun x : ivar => fun sigma : substitution => fun M : tm => forallb (fun z : ivar => negb (isFreeIn x (sigma z))) (getFVs M)
+  .
 
-Fixpoint run_substitution_on_tm (sigma : substitution) (M : tm) {struct M} : tm :=
-  match M with
-  | tmVar x => sigma x
-  | tmApp P1 P2 => tmApp (run_substitution_on_tm sigma P1) (run_substitution_on_tm sigma P2)
-  | tmLam y Q =>
-    let z : ivar := chi sigma M in
-    tmLam z (run_substitution_on_tm (cons_substitution y (tmVar z) sigma) Q)
-  end
-.
+  Definition chi : substitution -> tm -> ivar :=
+    fun sigma : substitution => fun M : tm => S (fold_right_max_0 (map (fun x : ivar => get_max_ivar (sigma x)) (getFVs M)))
+  .
 
-Theorem main_property_isFreshIn_substitution :
-  forall M : tm,
-  forall z : ivar,
-  forall sigma : substitution,
-  isFreshIn_substitution z sigma M = true <-> isFreeIn z (run_substitution_on_tm sigma M) = false.
-Proof with try now firstorder.
-  induction M; simpl.
-  - intros z sigma.
+  Theorem main_property_of_chi :
+    forall M : tm,
+    forall sigma : substitution,
+    isFreshIn_substitution (chi sigma M) sigma M = true.
+  Proof with try now firstorder.
+    assert ( claim1 :
+      forall sigma : substitution,
+      forall M : tm,
+      forall x : ivar,
+      isFreeIn x M = true ->
+      isFreeIn (chi sigma M) (sigma x) = false
+    ).
+    { intros sigma M x H.
+      enough (get_max_ivar (sigma x) < chi sigma M) by now apply get_max_ivar_lt.
+      unfold chi, fold_right_max_0.
+      enough (fold_right max 0 (map (fun z : ivar => get_max_ivar (sigma z)) (getFVs M)) >= get_max_ivar (sigma x)) by lia.
+      rewrite <- getFVs_isFreeIn in H.
+      apply fold_right_max_0_in, in_map_iff...
+    }
     unfold isFreshIn_substitution.
-    simpl.
-    rewrite andb_true_iff, negb_true_iff...
-  - intros z sigma.
-    rewrite orb_false_iff.
-    unfold isFreshIn_substitution.
-    simpl.
-    rewrite forallb_app, andb_true_iff...
-  - intros z sigma.
-    rewrite andb_false_iff, negb_false_iff, Nat.eqb_eq.
-    unfold isFreshIn_substitution.
-    simpl.
-    rewrite forallb_true_iff.
-    split; intros H.
-    + destruct (ivar_eq_dec z (chi sigma (tmLam y M)))...
-      left.
-      apply IHM.
+    intros M sigma.
+    apply forallb_true_iff.
+    intros x H.
+    apply negb_true_iff, claim1, getFVs_isFreeIn...
+  Qed.
+
+  Lemma chi_nil : 
+    forall M : tm,
+    isFreeIn (chi nil_subtitution M) M = false.
+  Proof with try now firstorder.
+    intros M.
+    assert (H : isFreshIn_substitution (chi nil_subtitution M) nil_subtitution M = true) by apply main_property_of_chi.
+    unfold isFreshIn_substitution in H.
+    rewrite forallb_true_iff in H.
+    simpl in H.
+    apply not_true_iff_false.
+    intros H0.
+    assert (H1 : negb (chi nil_subtitution M =? chi nil_subtitution M) = true) by now apply H, getFVs_isFreeIn.
+    rewrite negb_true_iff, Nat.eqb_neq in H1...
+  Qed.
+
+  Fixpoint run_substitution_on_tm (sigma : substitution) (M : tm) {struct M} : tm :=
+    match M with
+    | tmVar x => sigma x
+    | tmApp P1 P2 => tmApp (run_substitution_on_tm sigma P1) (run_substitution_on_tm sigma P2)
+    | tmLam y Q =>
+      let z : ivar := chi sigma M in
+      tmLam z (run_substitution_on_tm (cons_substitution y (tmVar z) sigma) Q)
+    end
+  .
+
+  Theorem main_property_isFreshIn_substitution :
+    forall M : tm,
+    forall z : ivar,
+    forall sigma : substitution,
+    isFreshIn_substitution z sigma M = true <-> isFreeIn z (run_substitution_on_tm sigma M) = false.
+  Proof with try now firstorder.
+    induction M; simpl.
+    - intros z sigma.
       unfold isFreshIn_substitution.
+      simpl.
+      rewrite andb_true_iff, negb_true_iff...
+    - intros z sigma.
+      rewrite orb_false_iff.
+      unfold isFreshIn_substitution.
+      simpl.
+      rewrite forallb_app, andb_true_iff...
+    - intros z sigma.
+      rewrite andb_false_iff, negb_false_iff, Nat.eqb_eq.
+      unfold isFreshIn_substitution.
+      simpl.
       rewrite forallb_true_iff.
-      intros x H0.
-      unfold cons_substitution.
-      destruct (ivar_eq_dec y x).
-      * unfold isFreeIn.
-        apply negb_true_iff, Nat.eqb_neq...
-      * apply H, in_in_remove...
-    + intros x H0.
-      apply in_remove in H0.
-      destruct H0.
-      destruct H.
-      * assert (H2 : isFreshIn_substitution z (cons_substitution y (tmVar (chi sigma (tmLam y M))) sigma) M = true) by now apply IHM.
-        unfold isFreshIn_substitution in H2.
-        rewrite forallb_true_iff in H2.
-        assert (H3 := H2 x H0).
-        unfold cons_substitution in H3.
-        destruct (ivar_eq_dec y x)...
-      * assert (H2 : isFreshIn_substitution z sigma (tmLam y M) = true).
-        { rewrite H.
-          apply main_property_of_chi...
+      split; intros H.
+      + destruct (ivar_eq_dec z (chi sigma (tmLam y M)))...
+        left.
+        apply IHM.
+        unfold isFreshIn_substitution.
+        rewrite forallb_true_iff.
+        intros x H0.
+        unfold cons_substitution.
+        destruct (ivar_eq_dec y x).
+        * unfold isFreeIn.
+          apply negb_true_iff, Nat.eqb_neq...
+        * apply H, in_in_remove...
+      + intros x H0.
+        apply in_remove in H0.
+        destruct H0.
+        destruct H.
+        * assert (H2 : isFreshIn_substitution z (cons_substitution y (tmVar (chi sigma (tmLam y M))) sigma) M = true) by now apply IHM.
+          unfold isFreshIn_substitution in H2.
+          rewrite forallb_true_iff in H2.
+          assert (H3 := H2 x H0).
+          unfold cons_substitution in H3.
+          destruct (ivar_eq_dec y x)...
+        * assert (H2 : isFreshIn_substitution z sigma (tmLam y M) = true).
+          { rewrite H.
+            apply main_property_of_chi...
+          }
+          unfold isFreshIn_substitution in H2.
+          rewrite forallb_true_iff in H2.
+          apply H2.
+          rewrite getFVs_isFreeIn.
+          simpl.
+          rewrite andb_true_iff, negb_true_iff, Nat.eqb_neq, <- getFVs_isFreeIn...
+  Qed.
+
+  Definition equiv_substitution_wrt : substitution -> substitution -> tm -> Prop :=
+    fun sigma1 : substitution => fun sigma2 : substitution => fun M : tm => forall x : ivar, isFreeIn x M = true -> sigma1 x = sigma2 x
+  .
+
+  Lemma property1_of_equiv_substitution_wrt :
+    forall sigma1 : substitution,
+    forall sigma2 : substitution,
+    (forall x : ivar, sigma1 x = sigma2 x) ->
+    forall M : tm,
+    equiv_substitution_wrt sigma1 sigma2 M.
+  Proof with try now firstorder.
+    unfold equiv_substitution_wrt...
+  Qed.
+
+  Lemma chi_equiv_substitution_wrt :
+    forall sigma1 : substitution,
+    forall sigma2 : substitution,
+    forall M : tm,
+    equiv_substitution_wrt sigma1 sigma2 M ->
+    chi sigma1 M = chi sigma2 M.
+  Proof with reflexivity.
+    unfold chi.
+    intros sigma1 sigma2 M H.
+    enough (H0 : (map (fun x : ivar => get_max_ivar (sigma1 x)) (getFVs M)) = (map (fun x : ivar => get_max_ivar (sigma2 x)) (getFVs M))) by congruence.
+    apply map_ext_in.
+    intros x H0.
+    rewrite (H x (proj1 (getFVs_isFreeIn M x) H0))...
+  Qed.
+
+  Theorem main_property_of_equiv_substitution_wrt :
+    forall M : tm,
+    forall sigma1 : substitution,
+    forall sigma2 : substitution,
+    equiv_substitution_wrt sigma1 sigma2 M ->
+    run_substitution_on_tm sigma1 M = run_substitution_on_tm sigma2 M.
+  Proof with try now firstorder.
+    induction M.
+    - intros sigma1 sigma2 H.
+      apply H.
+      simpl.
+      rewrite Nat.eqb_eq...
+    - intros sigma1 sigma2 H.
+      assert (H1 : equiv_substitution_wrt sigma1 sigma2 M1).
+      { intros x H0.
+        apply H.
+        simpl.
+        rewrite orb_true_iff...
+      }
+      assert (H2 : equiv_substitution_wrt sigma1 sigma2 M2).
+      { intros x H0.
+        apply H.
+        simpl.
+        rewrite orb_true_iff...
+      }
+      simpl.
+      rewrite (IHM1 sigma1 sigma2 H1), (IHM2 sigma1 sigma2 H2)...
+    - intros sigma1 sigma2 H.
+      simpl.
+      assert (H0 : equiv_substitution_wrt (cons_substitution y (tmVar (chi sigma1 (tmLam y M))) sigma1) (cons_substitution y (tmVar (chi sigma2 (tmLam y M))) sigma2) M).
+      { intros x H0.
+        unfold cons_substitution.
+        destruct (ivar_eq_dec y x).
+        - rewrite (chi_equiv_substitution_wrt sigma1 sigma2 (tmLam y M) H)...
+        - apply H.
+          simpl.
+          rewrite andb_true_iff, negb_true_iff, Nat.eqb_neq...
+      }
+      assert (H1 : chi sigma1 (tmLam y M) = chi sigma2 (tmLam y M)) by now apply chi_equiv_substitution_wrt.
+      rewrite (IHM (cons_substitution y (tmVar (chi sigma1 (tmLam y M))) sigma1) (cons_substitution y (tmVar (chi sigma2 (tmLam y M))) sigma2) H0), H1...
+  Qed.
+
+  Lemma trivial_substitution :
+    forall x : ivar,
+    forall M : tm,
+    run_substitution_on_tm (cons_substitution x (tmVar x) nil_subtitution) M = run_substitution_on_tm nil_subtitution M.
+  Proof with try now firstorder.
+    unfold cons_substitution.
+    intros x M.
+    apply main_property_of_equiv_substitution_wrt.
+    intros y H.
+    destruct (ivar_eq_dec x y)...
+  Qed.
+
+  Definition compose_substitution : substitution -> substitution -> substitution :=
+    fun sigma1 : substitution => fun sigma2 : substitution => fun x : ivar => run_substitution_on_tm sigma1 (sigma2 x)
+  .
+
+  Lemma distri_compose_cons :
+    forall M : tm,
+    forall N : tm,
+    forall sigma1 : substitution,
+    forall sigma2 : substitution,
+    forall x : ivar,
+    forall y : ivar,
+    isFreshIn_substitution y sigma1 (tmLam x M) = true ->
+    forall z : ivar,
+    isFreeIn z M = true ->
+    cons_substitution x N (compose_substitution sigma2 sigma1) z = compose_substitution (cons_substitution y N sigma2) (cons_substitution x (tmVar y) sigma1) z.
+  Proof with try now firstorder.
+    intros M N sigma1 sigma2 x y H z H0.
+    unfold cons_substitution, compose_substitution.
+    destruct (ivar_eq_dec x z).
+    - simpl.
+      destruct (ivar_eq_dec y y)...
+    - unfold isFreshIn_substitution in H.
+      rewrite forallb_true_iff in H.
+      assert (H1 : isFreeIn y (sigma1 z) = false).
+      { apply negb_true_iff, H, getFVs_isFreeIn.
+        simpl.
+        rewrite andb_true_iff, negb_true_iff, Nat.eqb_neq...
+      }
+      assert ( claim1 :
+        forall u : ivar,
+        isFreeIn u (sigma1 z) = true ->
+        cons_substitution y N sigma2 u = sigma2 u
+      ).
+      { unfold cons_substitution.
+        intros u H2.
+        destruct (ivar_eq_dec y u)...
+        subst.
+        rewrite H1 in H2...
+      }
+      apply main_property_of_equiv_substitution_wrt...
+  Qed.
+
+  Corollary distri_compose_cons_for_chi :
+    forall M : tm,
+    forall N : tm,
+    forall sigma1 : substitution,
+    forall sigma2 : substitution,
+    forall x : ivar,
+    let y : ivar := chi sigma1 (tmLam x M) in
+    forall z : ivar,
+    isFreeIn z M = true ->
+    cons_substitution x N (compose_substitution sigma2 sigma1) z = compose_substitution (cons_substitution y N sigma2) (cons_substitution x (tmVar y) sigma1) z.
+  Proof with eauto using distri_compose_cons, main_property_of_chi.
+    intros M N sigma1 sigma2 x y z H...
+  Qed.
+
+  Definition FreeIn_wrt : ivar -> substitution -> tm -> Prop :=
+    fun x : ivar => fun sigma : substitution => fun M : tm => exists y : ivar, isFreeIn y M = true /\ isFreeIn x (sigma y) = true
+  .
+
+  Theorem isFreeIn_wrt_true_iff (M : tm) :
+    forall z : ivar,
+    forall sigma : substitution,
+    isFreeIn z (run_substitution_on_tm sigma M) = true <-> FreeIn_wrt z sigma M.
+  Proof with try now firstorder.
+    unfold FreeIn_wrt.
+    induction M; simpl.
+    - intros z sigma.
+      split; intros H.
+      + exists x.
+        rewrite Nat.eqb_eq...
+      + destruct H as [y H].
+        rewrite Nat.eqb_eq in H.
+        destruct H.
+        subst...
+    - intros z sigma.
+      rewrite orb_true_iff.
+      split; intros H.
+      + destruct H; [enough (H0 : exists y : ivar, isFreeIn y M1 = true /\ isFreeIn z (sigma y) = true) | enough (H0 : exists y : ivar, isFreeIn y M2 = true /\ isFreeIn z (sigma y) = true)]...
+        all: destruct H0 as [y]; exists y; rewrite orb_true_iff...
+      + destruct H as [y].
+        rewrite orb_true_iff in H...
+    - intros x sigma.
+      rewrite andb_true_iff, negb_true_iff, Nat.eqb_neq.
+      split; intros H.
+      + destruct H.
+        assert (H1 := proj1 (IHM x (cons_substitution y (tmVar (chi sigma (tmLam y M))) sigma)) H).
+        destruct H1 as [w].
+        destruct H1.
+        set (z := chi sigma (tmLam y M)).
+        fold z in H, H0, H2.
+        destruct (ivar_eq_dec y w).
+        * subst.
+          unfold cons_substitution in H2.
+          destruct (ivar_eq_dec w w)...
+          unfold isFreeIn in H2.
+          rewrite Nat.eqb_eq in H2...
+        * exists w.
+          rewrite andb_true_iff, negb_true_iff, Nat.eqb_neq.
+          unfold cons_substitution in H2.
+          destruct (ivar_eq_dec y w)...
+      + rename y into z.
+        destruct H as [y].
+        destruct H.
+        set (w := chi sigma (tmLam z M)).
+        rewrite andb_true_iff, negb_true_iff, Nat.eqb_neq in H.
+        destruct (ivar_eq_dec w x).
+        * subst.
+          assert (isFreshIn_substitution w sigma (tmLam z M) = true) by now apply main_property_of_chi.
+          unfold isFreshIn_substitution in H1.
+          rewrite forallb_true_iff in H1.
+          enough (H2 : isFreeIn w (sigma y) = false) by now rewrite H0 in H2.
+          apply negb_true_iff, H1, getFVs_isFreeIn.
+          simpl.
+          rewrite andb_true_iff, negb_true_iff, Nat.eqb_neq...
+        * split...
+          apply IHM.
+          exists y.
+          split...
+          unfold cons_substitution.
+          destruct (ivar_eq_dec z y)...
+  Qed.
+
+  Lemma chi_ext :
+    forall sigma : substitution,
+    forall sigma' : substitution,
+    forall M : tm,
+    forall M' : tm,
+    (forall z : ivar, FreeIn_wrt z sigma M <-> FreeIn_wrt z sigma' M') ->
+    chi sigma M = chi sigma' M'.
+  Proof with try now firstorder.
+    unfold chi, FreeIn_wrt.
+    intros.
+    enough (fold_right_max_0 (map (fun x : ivar => get_max_ivar (sigma x)) (getFVs M)) = fold_right_max_0 (map (fun x : ivar => get_max_ivar (sigma' x)) (getFVs M'))) by lia.
+    assert ( claim1 :
+      forall z : ivar,
+      In z (flat_map (fun y : ivar => getFVs (sigma y)) (getFVs M)) <-> In z (flat_map (fun y : ivar => getFVs (sigma' y)) (getFVs M'))
+    ).
+    { intros z.
+      repeat (rewrite in_flat_map).
+      split; intros.
+      all: destruct H0 as [x]; rewrite getFVs_isFreeIn in H0.
+      1: assert (H1 : exists y : ivar, isFreeIn y M' = true /\ isFreeIn z (sigma' y) = true).
+      3: assert (H1 : exists y : ivar, isFreeIn y M = true /\ isFreeIn z (sigma y) = true).
+      1, 3: apply H; exists x...
+      1, 2: rewrite getFVs_isFreeIn in H0...
+      all: destruct H1 as [y]; exists y; repeat (rewrite getFVs_isFreeIn)...
+    }
+    assert (H0 : fold_right_max_0 (flat_map (fun y : ivar => getFVs (sigma y)) (getFVs M)) = fold_right_max_0 (flat_map (fun y : ivar => getFVs (sigma' y)) (getFVs M'))) by now apply fold_right_max_0_ext.
+    unfold get_max_ivar.
+    enough (H1 : forall xs : list ivar, forall f : ivar -> list ivar, fold_right_max_0 (map (fun x : ivar => fold_right_max_0 (f x)) xs) = fold_right_max_0 (flat_map f xs)) by now repeat (rewrite H1).
+    induction xs; simpl; intros f...
+    rewrite fold_right_max_0_app...
+  Qed.
+
+  Theorem main_property_of_compose_substitution :
+    forall M : tm,
+    forall sigma1 : substitution,
+    forall sigma2 : substitution,
+    run_substitution_on_tm sigma2 (run_substitution_on_tm sigma1 M) = run_substitution_on_tm (compose_substitution sigma2 sigma1) M.
+  Proof with try now firstorder.
+    induction M; simpl.
+    - intros sigma1 sigma2...
+    - intros sigma1 sigma2.
+      rewrite IHM1, IHM2...
+    - intros sigma1 sigma2.
+      enough (lemma : chi sigma2 (run_substitution_on_tm sigma1 (tmLam y M)) = chi (compose_substitution sigma2 sigma1) (tmLam y M)).
+      { set (x := chi sigma1 (tmLam y M)).
+        set (x' := chi sigma2 (tmLam x (run_substitution_on_tm (cons_substitution y (tmVar x) sigma1) M))).
+        set (z := chi (compose_substitution sigma2 sigma1) (tmLam y M)).
+        assert (H := IHM (cons_substitution y (tmVar x) sigma1) (cons_substitution x (tmVar x') sigma2)).
+        rewrite H.
+        assert (H0 : run_substitution_on_tm (compose_substitution (cons_substitution x (tmVar x') sigma2) (cons_substitution y (tmVar x) sigma1)) M = run_substitution_on_tm (cons_substitution y (tmVar x') (compose_substitution sigma2 sigma1)) M).
+        { apply main_property_of_equiv_substitution_wrt.
+          intros u H0.
+          assert (H1 := distri_compose_cons_for_chi M (tmVar x') sigma1 sigma2 y).
+          simpl in H1.
+          rewrite (H1 u H0)...
         }
-        unfold isFreshIn_substitution in H2.
-        rewrite forallb_true_iff in H2.
-        apply H2.
+        rewrite H0.
+        replace x' with z...
+      }
+      rename y into x.
+      set (y := chi sigma1 (tmLam x M)).
+      assert ( claim1 :
+        forall y' : ivar,
+        (exists x' : ivar, isFreeIn x' (tmLam y (run_substitution_on_tm (cons_substitution x (tmVar y) sigma1) M)) = true /\ isFreeIn y' (sigma2 x') = true) ->
+        (exists u : ivar, isFreeIn u (tmLam x M) = true /\ isFreeIn y' (compose_substitution sigma2 sigma1 u) = true)
+      ).
+      { intros y' H.
+        destruct H as [x'].
+        destruct H.
+        simpl in H.
+        rewrite andb_true_iff, negb_true_iff, Nat.eqb_neq in H.
+        destruct H.
+        assert (H2 := proj1 (isFreeIn_wrt_true_iff M x' (cons_substitution x (tmVar y) sigma1)) H).
+        destruct H2 as [u].
+        destruct H2.
+        unfold cons_substitution in H3.
+        destruct (ivar_eq_dec x u).
+        - unfold isFreeIn in H3.
+          rewrite Nat.eqb_eq in H3...
+        - exists u.
+          split.
+          + simpl.
+            rewrite andb_true_iff, negb_true_iff, Nat.eqb_neq...
+          + apply (proj2 (isFreeIn_wrt_true_iff (sigma1 u) y' sigma2))...
+      }
+      assert ( claim2 :
+        forall y' : ivar,
+        (exists x' : ivar, isFreeIn x' (tmLam x M) = true /\ isFreeIn y' (compose_substitution sigma2 sigma1 x') = true) ->
+        (exists u : ivar, isFreeIn u (tmLam y (run_substitution_on_tm (cons_substitution x (tmVar y) sigma1) M)) = true /\ isFreeIn y' (sigma2 u) = true)
+      ).
+      { intros y' H.
+        destruct H as [x'].
+        destruct H.
+        simpl in H.
+        rewrite andb_true_iff, negb_true_iff, Nat.eqb_neq in H.
+        destruct H.
+        assert (H2 := proj1 (isFreeIn_wrt_true_iff (sigma1 x') y' sigma2) H0).
+        destruct H2 as [u].
+        destruct H2.
+        assert (H4 : isFreeIn u (run_substitution_on_tm (cons_substitution x (tmVar y) sigma1) M) = true).
+        { apply isFreeIn_wrt_true_iff.
+          exists x'.
+          split...
+          unfold cons_substitution.
+          destruct (ivar_eq_dec x x')...
+        }
+        exists u.
+        split...
+        simpl.
+        rewrite andb_true_iff, negb_true_iff, Nat.eqb_neq.
+        split...
+        intros H5.
+        subst.
+        enough (H6 : isFreeIn y (sigma1 x') = false) by now rewrite H2 in H6.
+        assert (H5 := main_property_of_chi (tmLam x M) sigma1).
+        unfold isFreshIn_substitution in H5.
+        rewrite forallb_true_iff in H5.
+        apply negb_true_iff, H5.
         rewrite getFVs_isFreeIn.
         simpl.
-        rewrite andb_true_iff, negb_true_iff, Nat.eqb_neq, <- getFVs_isFreeIn...
-Qed.
-
-Definition equiv_substitution_wrt : substitution -> substitution -> tm -> Prop :=
-  fun sigma1 : substitution => fun sigma2 : substitution => fun M : tm => forall x : ivar, isFreeIn x M = true -> sigma1 x = sigma2 x
-.
-
-Lemma property1_of_equiv_substitution_wrt :
-  forall sigma1 : substitution,
-  forall sigma2 : substitution,
-  (forall x : ivar, sigma1 x = sigma2 x) ->
-  forall M : tm,
-  equiv_substitution_wrt sigma1 sigma2 M.
-Proof with try now firstorder.
-  unfold equiv_substitution_wrt...
-Qed.
-
-Lemma chi_equiv_substitution_wrt :
-  forall sigma1 : substitution,
-  forall sigma2 : substitution,
-  forall M : tm,
-  equiv_substitution_wrt sigma1 sigma2 M ->
-  chi sigma1 M = chi sigma2 M.
-Proof with reflexivity.
-  unfold chi.
-  intros sigma1 sigma2 M H.
-  enough (H0 : (map (fun x : ivar => get_max_ivar (sigma1 x)) (getFVs M)) = (map (fun x : ivar => get_max_ivar (sigma2 x)) (getFVs M))) by congruence.
-  apply map_ext_in.
-  intros x H0.
-  rewrite (H x (proj1 (getFVs_isFreeIn M x) H0))...
-Qed.
-
-Theorem main_property_of_equiv_substitution_wrt :
-  forall M : tm,
-  forall sigma1 : substitution,
-  forall sigma2 : substitution,
-  equiv_substitution_wrt sigma1 sigma2 M ->
-  run_substitution_on_tm sigma1 M = run_substitution_on_tm sigma2 M.
-Proof with try now firstorder.
-  induction M.
-  - intros sigma1 sigma2 H.
-    apply H.
-    simpl.
-    rewrite Nat.eqb_eq...
-  - intros sigma1 sigma2 H.
-    assert (H1 : equiv_substitution_wrt sigma1 sigma2 M1).
-    { intros x H0.
-      apply H.
-      simpl.
-      rewrite orb_true_iff...
-    }
-    assert (H2 : equiv_substitution_wrt sigma1 sigma2 M2).
-    { intros x H0.
-      apply H.
-      simpl.
-      rewrite orb_true_iff...
-    }
-    simpl.
-    rewrite (IHM1 sigma1 sigma2 H1), (IHM2 sigma1 sigma2 H2)...
-  - intros sigma1 sigma2 H.
-    simpl.
-    assert (H0 : equiv_substitution_wrt (cons_substitution y (tmVar (chi sigma1 (tmLam y M))) sigma1) (cons_substitution y (tmVar (chi sigma2 (tmLam y M))) sigma2) M).
-    { intros x H0.
-      unfold cons_substitution.
-      destruct (ivar_eq_dec y x).
-      - rewrite (chi_equiv_substitution_wrt sigma1 sigma2 (tmLam y M) H)...
-      - apply H.
-        simpl.
         rewrite andb_true_iff, negb_true_iff, Nat.eqb_neq...
-    }
-    assert (H1 : chi sigma1 (tmLam y M) = chi sigma2 (tmLam y M)) by now apply chi_equiv_substitution_wrt.
-    rewrite (IHM (cons_substitution y (tmVar (chi sigma1 (tmLam y M))) sigma1) (cons_substitution y (tmVar (chi sigma2 (tmLam y M))) sigma2) H0), H1...
-Qed.
+      }
+      apply chi_ext...
+  Qed.
 
-Lemma trivial_substitution :
-  forall x : ivar,
-  forall M : tm,
-  run_substitution_on_tm (cons_substitution x (tmVar x) nil_subtitution) M = run_substitution_on_tm nil_subtitution M.
-Proof with try now firstorder.
-  unfold cons_substitution.
-  intros x M.
-  apply main_property_of_equiv_substitution_wrt.
-  intros y H.
-  destruct (ivar_eq_dec x y)...
-Qed.
+  Corollary compose_one :
+    forall M : tm,
+    forall N : tm,
+    forall sigma : substitution,
+    forall x : ivar,
+    run_substitution_on_tm (cons_substitution x (run_substitution_on_tm sigma N) sigma) M = run_substitution_on_tm sigma (run_substitution_on_tm (cons_substitution x N nil_subtitution) M).
+  Proof with try now firstorder.
+    intros M N sigma x.
+    replace (run_substitution_on_tm (cons_substitution x (run_substitution_on_tm sigma N) sigma) M) with (run_substitution_on_tm (cons_substitution x (run_substitution_on_tm sigma N) (compose_substitution sigma nil_subtitution)) M).
+    replace (run_substitution_on_tm (cons_substitution x (run_substitution_on_tm sigma N) (compose_substitution sigma nil_subtitution)) M) with (run_substitution_on_tm (compose_substitution sigma (cons_substitution x N nil_subtitution)) M).
+    rewrite main_property_of_compose_substitution...
+    all: apply main_property_of_equiv_substitution_wrt; apply property1_of_equiv_substitution_wrt; unfold compose_substitution, cons_substitution, nil_subtitution; intros z; destruct (ivar_eq_dec x z)...
+  Qed.
 
-Definition compose_substitution : substitution -> substitution -> substitution :=
-  fun sigma1 : substitution => fun sigma2 : substitution => fun x : ivar => run_substitution_on_tm sigma1 (sigma2 x)
-.
-
-Lemma distri_compose_cons :
-  forall M : tm,
-  forall N : tm,
-  forall sigma1 : substitution,
-  forall sigma2 : substitution,
-  forall x : ivar,
-  forall y : ivar,
-  isFreshIn_substitution y sigma1 (tmLam x M) = true ->
-  forall z : ivar,
-  isFreeIn z M = true ->
-  cons_substitution x N (compose_substitution sigma2 sigma1) z = compose_substitution (cons_substitution y N sigma2) (cons_substitution x (tmVar y) sigma1) z.
-Proof with try now firstorder.
-  intros M N sigma1 sigma2 x y H z H0.
-  unfold cons_substitution, compose_substitution.
-  destruct (ivar_eq_dec x z).
-  - simpl.
-    destruct (ivar_eq_dec y y)...
-  - unfold isFreshIn_substitution in H.
-    rewrite forallb_true_iff in H.
-    assert (H1 : isFreeIn y (sigma1 z) = false).
-    { apply negb_true_iff, H, getFVs_isFreeIn.
-      simpl.
-      rewrite andb_true_iff, negb_true_iff, Nat.eqb_neq...
-    }
-    assert ( claim1 :
-      forall u : ivar,
-      isFreeIn u (sigma1 z) = true ->
-      cons_substitution y N sigma2 u = sigma2 u
-    ).
-    { unfold cons_substitution.
-      intros u H2.
-      destruct (ivar_eq_dec y u)...
-      subst.
-      rewrite H1 in H2...
-    }
-    apply main_property_of_equiv_substitution_wrt...
-Qed.
-
-Corollary distri_compose_cons_for_chi :
-  forall M : tm,
-  forall N : tm,
-  forall sigma1 : substitution,
-  forall sigma2 : substitution,
-  forall x : ivar,
-  let y : ivar := chi sigma1 (tmLam x M) in
-  forall z : ivar,
-  isFreeIn z M = true ->
-  cons_substitution x N (compose_substitution sigma2 sigma1) z = compose_substitution (cons_substitution y N sigma2) (cons_substitution x (tmVar y) sigma1) z.
-Proof with eauto using distri_compose_cons, main_property_of_chi.
-  intros M N sigma1 sigma2 x y z H...
-Qed.
-
-Definition FreeIn_wrt : ivar -> substitution -> tm -> Prop :=
-  fun x : ivar => fun sigma : substitution => fun M : tm => exists y : ivar, isFreeIn y M = true /\ isFreeIn x (sigma y) = true
-.
-
-Theorem isFreeIn_wrt_true_iff (M : tm) :
-  forall z : ivar,
-  forall sigma : substitution,
-  isFreeIn z (run_substitution_on_tm sigma M) = true <-> FreeIn_wrt z sigma M.
-Proof with try now firstorder.
-  unfold FreeIn_wrt.
-  induction M; simpl.
-  - intros z sigma.
-    split; intros H.
-    + exists x.
-      rewrite Nat.eqb_eq...
-    + destruct H as [y H].
-      rewrite Nat.eqb_eq in H.
-      destruct H.
-      subst...
-  - intros z sigma.
-    rewrite orb_true_iff.
-    split; intros H.
-    + destruct H; [enough (H0 : exists y : ivar, isFreeIn y M1 = true /\ isFreeIn z (sigma y) = true) | enough (H0 : exists y : ivar, isFreeIn y M2 = true /\ isFreeIn z (sigma y) = true)]...
-      all: destruct H0 as [y]; exists y; rewrite orb_true_iff...
-    + destruct H as [y].
-      rewrite orb_true_iff in H...
-  - intros x sigma.
-    rewrite andb_true_iff, negb_true_iff, Nat.eqb_neq.
-    split; intros H.
-    + destruct H.
-      assert (H1 := proj1 (IHM x (cons_substitution y (tmVar (chi sigma (tmLam y M))) sigma)) H).
-      destruct H1 as [w].
-      destruct H1.
-      set (z := chi sigma (tmLam y M)).
-      fold z in H, H0, H2.
-      destruct (ivar_eq_dec y w).
-      * subst.
-        unfold cons_substitution in H2.
-        destruct (ivar_eq_dec w w)...
-        unfold isFreeIn in H2.
-        rewrite Nat.eqb_eq in H2...
-      * exists w.
-        rewrite andb_true_iff, negb_true_iff, Nat.eqb_neq.
-        unfold cons_substitution in H2.
-        destruct (ivar_eq_dec y w)...
-    + rename y into z.
-      destruct H as [y].
-      destruct H.
-      set (w := chi sigma (tmLam z M)).
-      rewrite andb_true_iff, negb_true_iff, Nat.eqb_neq in H.
-      destruct (ivar_eq_dec w x).
-      * subst.
-        assert (isFreshIn_substitution w sigma (tmLam z M) = true) by now apply main_property_of_chi.
-        unfold isFreshIn_substitution in H1.
-        rewrite forallb_true_iff in H1.
-        enough (H2 : isFreeIn w (sigma y) = false) by now rewrite H0 in H2.
-        apply negb_true_iff, H1, getFVs_isFreeIn.
-        simpl.
-        rewrite andb_true_iff, negb_true_iff, Nat.eqb_neq...
-      * split...
-        apply IHM.
-        exists y.
-        split...
-        unfold cons_substitution.
-        destruct (ivar_eq_dec z y)...
-Qed.
-
-Lemma chi_ext :
-  forall sigma : substitution,
-  forall sigma' : substitution,
-  forall M : tm,
-  forall M' : tm,
-  (forall z : ivar, FreeIn_wrt z sigma M <-> FreeIn_wrt z sigma' M') ->
-  chi sigma M = chi sigma' M'.
-Proof with try now firstorder.
-  unfold chi, FreeIn_wrt.
-  intros.
-  enough (fold_right_max_0 (map (fun x : ivar => get_max_ivar (sigma x)) (getFVs M)) = fold_right_max_0 (map (fun x : ivar => get_max_ivar (sigma' x)) (getFVs M'))) by lia.
-  assert ( claim1 :
+  Theorem main_property_of_cons_substitution :
+    forall x : ivar,
     forall z : ivar,
-    In z (flat_map (fun y : ivar => getFVs (sigma y)) (getFVs M)) <-> In z (flat_map (fun y : ivar => getFVs (sigma' y)) (getFVs M'))
-  ).
-  { intros z.
-    repeat (rewrite in_flat_map).
-    split; intros.
-    all: destruct H0 as [x]; rewrite getFVs_isFreeIn in H0.
-    1: assert (H1 : exists y : ivar, isFreeIn y M' = true /\ isFreeIn z (sigma' y) = true).
-    3: assert (H1 : exists y : ivar, isFreeIn y M = true /\ isFreeIn z (sigma y) = true).
-    1, 3: apply H; exists x...
-    1, 2: rewrite getFVs_isFreeIn in H0...
-    all: destruct H1 as [y]; exists y; repeat (rewrite getFVs_isFreeIn)...
-  }
-  assert (H0 : fold_right_max_0 (flat_map (fun y : ivar => getFVs (sigma y)) (getFVs M)) = fold_right_max_0 (flat_map (fun y : ivar => getFVs (sigma' y)) (getFVs M'))) by now apply fold_right_max_0_ext.
-  unfold get_max_ivar.
-  enough (H1 : forall xs : list ivar, forall f : ivar -> list ivar, fold_right_max_0 (map (fun x : ivar => fold_right_max_0 (f x)) xs) = fold_right_max_0 (flat_map f xs)) by now repeat (rewrite H1).
-  induction xs; simpl; intros f...
-  rewrite fold_right_max_0_app...
-Qed.
-
-Theorem main_property_of_compose_substitution :
-  forall M : tm,
-  forall sigma1 : substitution,
-  forall sigma2 : substitution,
-  run_substitution_on_tm sigma2 (run_substitution_on_tm sigma1 M) = run_substitution_on_tm (compose_substitution sigma2 sigma1) M.
-Proof with try now firstorder.
-  induction M; simpl.
-  - intros sigma1 sigma2...
-  - intros sigma1 sigma2.
-    rewrite IHM1, IHM2...
-  - intros sigma1 sigma2.
-    enough (lemma : chi sigma2 (run_substitution_on_tm sigma1 (tmLam y M)) = chi (compose_substitution sigma2 sigma1) (tmLam y M)).
-    { set (x := chi sigma1 (tmLam y M)).
-      set (x' := chi sigma2 (tmLam x (run_substitution_on_tm (cons_substitution y (tmVar x) sigma1) M))).
-      set (z := chi (compose_substitution sigma2 sigma1) (tmLam y M)).
-      assert (H := IHM (cons_substitution y (tmVar x) sigma1) (cons_substitution x (tmVar x') sigma2)).
-      rewrite H.
-      assert (H0 : run_substitution_on_tm (compose_substitution (cons_substitution x (tmVar x') sigma2) (cons_substitution y (tmVar x) sigma1)) M = run_substitution_on_tm (cons_substitution y (tmVar x') (compose_substitution sigma2 sigma1)) M).
-      { apply main_property_of_equiv_substitution_wrt.
-        intros u H0.
-        assert (H1 := distri_compose_cons_for_chi M (tmVar x') sigma1 sigma2 y).
-        simpl in H1.
-        rewrite (H1 u H0)...
-      }
-      rewrite H0.
-      replace x' with z...
-    }
-    rename y into x.
-    set (y := chi sigma1 (tmLam x M)).
-    assert ( claim1 :
-      forall y' : ivar,
-      (exists x' : ivar, isFreeIn x' (tmLam y (run_substitution_on_tm (cons_substitution x (tmVar y) sigma1) M)) = true /\ isFreeIn y' (sigma2 x') = true) ->
-      (exists u : ivar, isFreeIn u (tmLam x M) = true /\ isFreeIn y' (compose_substitution sigma2 sigma1 u) = true)
-    ).
-    { intros y' H.
-      destruct H as [x'].
-      destruct H.
+    forall M : tm,
+    forall N : tm,
+    forall sigma : substitution,
+    isFreeIn z (tmLam x M) = false ->
+    run_substitution_on_tm (cons_substitution x N sigma) M = run_substitution_on_tm (cons_substitution z N sigma) (run_substitution_on_tm (cons_substitution x (tmVar z) nil_subtitution) M).
+  Proof with try now firstorder.
+    intros.
+    rewrite (main_property_of_compose_substitution M (cons_substitution x (tmVar z) nil_subtitution) (cons_substitution z N sigma)).
+    apply main_property_of_equiv_substitution_wrt.
+    intros w H0.
+    unfold cons_substitution, nil_subtitution, compose_substitution.
+    destruct (ivar_eq_dec x w); simpl.
+    - destruct (ivar_eq_dec z z)...
+    - destruct (ivar_eq_dec z w)...
       simpl in H.
-      rewrite andb_true_iff, negb_true_iff, Nat.eqb_neq in H.
-      destruct H.
-      assert (H2 := proj1 (isFreeIn_wrt_true_iff M x' (cons_substitution x (tmVar y) sigma1)) H).
-      destruct H2 as [u].
-      destruct H2.
-      unfold cons_substitution in H3.
-      destruct (ivar_eq_dec x u).
-      - unfold isFreeIn in H3.
-        rewrite Nat.eqb_eq in H3...
-      - exists u.
-        split.
-        + simpl.
-          rewrite andb_true_iff, negb_true_iff, Nat.eqb_neq...
-        + apply (proj2 (isFreeIn_wrt_true_iff (sigma1 u) y' sigma2))...
-    }
-    assert ( claim2 :
-      forall y' : ivar,
-      (exists x' : ivar, isFreeIn x' (tmLam x M) = true /\ isFreeIn y' (compose_substitution sigma2 sigma1 x') = true) ->
-      (exists u : ivar, isFreeIn u (tmLam y (run_substitution_on_tm (cons_substitution x (tmVar y) sigma1) M)) = true /\ isFreeIn y' (sigma2 u) = true)
-    ).
-    { intros y' H.
-      destruct H as [x'].
-      destruct H.
+      subst.
+      rewrite H0 in H.
       simpl in H.
-      rewrite andb_true_iff, negb_true_iff, Nat.eqb_neq in H.
-      destruct H.
-      assert (H2 := proj1 (isFreeIn_wrt_true_iff (sigma1 x') y' sigma2) H0).
-      destruct H2 as [u].
-      destruct H2.
-      assert (H4 : isFreeIn u (run_substitution_on_tm (cons_substitution x (tmVar y) sigma1) M) = true).
-      { apply isFreeIn_wrt_true_iff.
-        exists x'.
-        split...
-        unfold cons_substitution.
-        destruct (ivar_eq_dec x x')...
-      }
-      exists u.
-      split...
-      simpl.
-      rewrite andb_true_iff, negb_true_iff, Nat.eqb_neq.
-      split...
-      intros H5.
-      subst.
-      enough (H6 : isFreeIn y (sigma1 x') = false) by now rewrite H2 in H6.
-      assert (H5 := main_property_of_chi (tmLam x M) sigma1).
-      unfold isFreshIn_substitution in H5.
-      rewrite forallb_true_iff in H5.
-      apply negb_true_iff, H5.
-      rewrite getFVs_isFreeIn.
-      simpl.
-      rewrite andb_true_iff, negb_true_iff, Nat.eqb_neq...
+      rewrite negb_false_iff, Nat.eqb_eq in H.
+      contradiction n...
+  Qed.
+
+  Class isPreLambdaStructure (D : Type) : Type :=
+    { runApp : D -> (D -> D)
+    ; runLam : (D -> D) -> D
     }
-    apply chi_ext...
-Qed.
+  .
 
-Corollary compose_one :
-  forall M : tm,
-  forall N : tm,
-  forall sigma : substitution,
-  forall x : ivar,
-  run_substitution_on_tm (cons_substitution x (run_substitution_on_tm sigma N) sigma) M = run_substitution_on_tm sigma (run_substitution_on_tm (cons_substitution x N nil_subtitution) M).
-Proof with try now firstorder.
-  intros M N sigma x.
-  replace (run_substitution_on_tm (cons_substitution x (run_substitution_on_tm sigma N) sigma) M) with (run_substitution_on_tm (cons_substitution x (run_substitution_on_tm sigma N) (compose_substitution sigma nil_subtitution)) M).
-  replace (run_substitution_on_tm (cons_substitution x (run_substitution_on_tm sigma N) (compose_substitution sigma nil_subtitution)) M) with (run_substitution_on_tm (compose_substitution sigma (cons_substitution x N nil_subtitution)) M).
-  rewrite main_property_of_compose_substitution...
-  all: apply main_property_of_equiv_substitution_wrt; apply property1_of_equiv_substitution_wrt; unfold compose_substitution, cons_substitution, nil_subtitution; intros z; destruct (ivar_eq_dec x z)...
-Qed.
+  Lemma runApp_ext {D : Type} `{D_isPreLambdaStructure : isPreLambdaStructure D} :
+    forall v1 : D,
+    forall v2 : D,
+    forall v1' : D,
+    forall v2' : D,
+    v1 = v1' ->
+    v2 = v2' ->
+    runApp v1 v2 = runApp v1' v2'.
+  Proof.
+    congruence.
+  Qed.
 
-Theorem main_property_of_cons_substitution :
-  forall x : ivar,
-  forall z : ivar,
-  forall M : tm,
-  forall N : tm,
-  forall sigma : substitution,
-  isFreeIn z (tmLam x M) = false ->
-  run_substitution_on_tm (cons_substitution x N sigma) M = run_substitution_on_tm (cons_substitution z N sigma) (run_substitution_on_tm (cons_substitution x (tmVar z) nil_subtitution) M).
-Proof with try now firstorder.
-  intros.
-  rewrite (main_property_of_compose_substitution M (cons_substitution x (tmVar z) nil_subtitution) (cons_substitution z N sigma)).
-  apply main_property_of_equiv_substitution_wrt.
-  intros w H0.
-  unfold cons_substitution, nil_subtitution, compose_substitution.
-  destruct (ivar_eq_dec x w); simpl.
-  - destruct (ivar_eq_dec z z)...
-  - destruct (ivar_eq_dec z w)...
-    simpl in H.
-    subst.
-    rewrite H0 in H.
-    simpl in H.
-    rewrite negb_false_iff, Nat.eqb_eq in H.
-    contradiction n...
-Qed.
+  Global Hint Resolve runApp_ext : my_hints.
 
-End Substitution.
+  Lemma runLam_ext {D : Type} `{D_isPreLambdaStructure : isPreLambdaStructure D} :
+    forall vv : D -> D,
+    forall vv' : D -> D,
+    (forall v0 : D, vv v0 = vv' v0) ->
+    runLam vv = runLam vv'.
+  Proof.
+    intros vv vv' H.
+    apply functional_extensionality in H.
+    congruence.
+  Qed.
 
-#[global] Create HintDb semantics_of_ulc.
+  Global Hint Resolve runLam_ext : my_hints.
 
-Class isPreLambdaStructure (Dom : Set) : Type :=
-  { eqnDom : Dom -> Dom -> Prop
-  ; runApp : Dom -> (Dom -> Dom)
-  ; runLam : (Dom -> Dom) -> Dom
-  ; eqnDom_refl :
-    forall v1 : Dom,
-    eqnDom v1 v1
-  ; eqnDom_sym :
-    forall v1 : Dom,
-    forall v2 : Dom,
-    eqnDom v1 v2 ->
-    eqnDom v2 v1
-  ; eqnDom_trans :
-    forall v1 : Dom,
-    forall v2 : Dom,
-    forall v3 : Dom,
-    eqnDom v1 v2 ->
-    eqnDom v2 v3 ->
-    eqnDom v1 v3
-  ; runApp_ext :
-    forall v1 : Dom,
-    forall v1' : Dom,
-    forall v2 : Dom,
-    forall v2' : Dom,
-    eqnDom v1 v1' ->
-    eqnDom v2 v2' ->
-    eqnDom (runApp v1 v2) (runApp v1' v2')
-  ; runLam_ext :
-    forall vv : Dom -> Dom,
-    forall vv' : Dom -> Dom,
-    (forall v0 : Dom, eqnDom (vv v0) (vv' v0)) ->
-    eqnDom (runLam vv) (runLam vv')
-  }
-.
+  Definition eval_tm {D : Type} `{D_is_model : isPreLambdaStructure D} : (ivar -> D) -> tm -> D :=
+    fix eval_tm_fix (E : ivar -> D) (M : tm) {struct M} : D :=
+    match M with
+    | tmVar x => E x
+    | tmApp P1 P2 => runApp (eval_tm_fix E P1) (eval_tm_fix E P2)
+    | tmLam y Q => runLam (fun v : D => eval_tm_fix (fun z : ivar => if ivar_eq_dec y z then v else E z) Q)
+    end
+  .
 
-Local Notation "v1 =-= v2" := (eqnDom v1 v2) (at level 70, no associativity) : type_scope.
-
-#[global] Hint Resolve eqnDom_refl : semantics_of_ulc.
-
-#[global] Hint Resolve eqnDom_sym : semantics_of_ulc.
-
-#[global] Hint Resolve eqnDom_trans : semantics_of_ulc.
-
-#[global] Hint Resolve runApp_ext : semantics_of_ulc.
-
-#[global] Hint Resolve runLam_ext : semantics_of_ulc.
-
-Section PreLambdaStructure.
-
-Variable D : Set.
-
-Fixpoint eval_tm `{D_is_model : isPreLambdaStructure D} (E : ivar -> D) (M : tm) {struct M} : D :=
-  match M with
-  | tmVar x => E x
-  | tmApp P1 P2 => runApp (eval_tm E P1) (eval_tm E P2)
-  | tmLam y Q => runLam (fun v : D => eval_tm (fun z : ivar => if ivar_eq_dec y z then v else E z) Q)
-  end
-.
-
-Lemma eval_tm_ext `{D_is_model : isPreLambdaStructure D} :
-  forall M : tm,
-  forall E1 : ivar -> D,
-  forall E2 : ivar -> D,
-  (forall z : ivar, isFreeIn z M = true -> E1 z =-= E2 z) ->
-  eval_tm E1 M =-= eval_tm E2 M.
-Proof with try now firstorder with semantics_of_ulc.
-  induction M; simpl.
-  - intros E1 E2 H.
-    apply H.
-    rewrite Nat.eqb_eq...
-  - intros E1 E2 H.
-    apply runApp_ext; [apply IHM1 | apply IHM2].
-    all: intros z H0; apply H; rewrite orb_true_iff...
-  - intros E1 E2 H.
-    apply runLam_ext.
-    intros v.
-    apply (IHM (fun z : ivar => if ivar_eq_dec y z then v else E1 z) (fun z : ivar => if ivar_eq_dec y z then v else E2 z))...
-    intros z H0.
-    destruct (ivar_eq_dec y z)...
-    apply H.
-    rewrite andb_true_iff, negb_true_iff, Nat.eqb_neq...
-Qed.
-
-Theorem run_substitution_on_tm_preserves_eval_tm `{D_is_model : isPreLambdaStructure D} :
-  forall M : tm,
-  forall sigma : substitution,
-  forall E : ivar -> D,
-  eval_tm (fun z : ivar => eval_tm E (sigma z)) M =-= eval_tm E (run_substitution_on_tm sigma M).
-Proof with try now firstorder with semantics_of_ulc.
-  induction M.
-  - intros sigma E...
-  - intros sigma E.
-    simpl...
-  - intros sigma E.
-    enough (claim1 : forall v : D, eval_tm (fun z : ivar => if ivar_eq_dec y z then v else eval_tm E (sigma z)) M =-= eval_tm (fun z : ivar => if ivar_eq_dec (chi sigma (tmLam y M)) z then v else E z) (run_substitution_on_tm (cons_substitution y (tmVar (chi sigma (tmLam y M))) sigma) M)) by now apply runLam_ext.
-    intros v.
-    assert (H := IHM (cons_substitution y (tmVar (chi sigma (tmLam y M))) sigma) (fun z : ivar => if ivar_eq_dec (chi sigma (tmLam y M)) z then v else E z)).
-    apply eqnDom_sym in H.
-    apply eqnDom_sym, (eqnDom_trans _ _ _ H), eval_tm_ext.
-    intros z H0.
-    unfold cons_substitution.
-    destruct (ivar_eq_dec y z).
-    + unfold eval_tm.
-      destruct (ivar_eq_dec (chi sigma (tmLam y M)) (chi sigma (tmLam y M)))...
-    + apply eval_tm_ext.
-      intros z' H1.
-      destruct (ivar_eq_dec (chi sigma (tmLam y M)) z')...
-      subst.
-      assert (H2 : isFreshIn_substitution (chi sigma (tmLam y M)) sigma (tmLam y M) = true) by now apply main_property_of_chi.
-      unfold isFreshIn_substitution in H2.
-      rewrite forallb_true_iff in H2.
-      enough (H3 : isFreeIn (chi sigma (tmLam y M)) (sigma z) = false) by now rewrite H3 in H1.
-      apply negb_true_iff, H2, getFVs_isFreeIn.
-      simpl.
+  Lemma eval_tm_ext {D : Type} `{D_is_model : isPreLambdaStructure D} :
+    forall M : tm,
+    forall E1 : ivar -> D,
+    forall E2 : ivar -> D,
+    (forall z : ivar, isFreeIn z M = true -> E1 z = E2 z) ->
+    eval_tm E1 M = eval_tm E2 M.
+  Proof with try now eauto with *.
+    induction M; simpl.
+    - intros E1 E2 H.
+      apply H.
+      rewrite Nat.eqb_eq...
+    - intros E1 E2 H.
+      rewrite (IHM1 E1 E2), (IHM2 E1 E2)...
+    - intros E1 E2 H.
+      enough (XXX : (fun v : D => eval_tm (fun z : ivar => if ivar_eq_dec y z then v else E1 z) M) = (fun v : D => eval_tm (fun z : ivar => if ivar_eq_dec y z then v else E2 z) M)) by congruence.
+      apply functional_extensionality.
+      intros v.
+      apply (IHM (fun z : ivar => if ivar_eq_dec y z then v else E1 z) (fun z : ivar => if ivar_eq_dec y z then v else E2 z))...
+      intros z H0.
+      destruct (ivar_eq_dec y z)...
+      apply H.
       rewrite andb_true_iff, negb_true_iff, Nat.eqb_neq...
-Qed.
+  Qed.
 
-End PreLambdaStructure.
+  Theorem run_substitution_on_tm_preserves_eval_tm {D : Type} `{D_is_model : isPreLambdaStructure D} :
+    forall M : tm,
+    forall sigma : substitution,
+    forall E : ivar -> D,
+    eval_tm (fun z : ivar => eval_tm E (sigma z)) M = eval_tm E (run_substitution_on_tm sigma M).
+  Proof with try now eauto with *.
+    induction M.
+    - intros sigma E...
+    - intros sigma E.
+      simpl...
+    - intros sigma E.
+      enough (claim1 : forall v : D, eval_tm (fun z : ivar => if ivar_eq_dec y z then v else eval_tm E (sigma z)) M = eval_tm (fun z : ivar => if ivar_eq_dec (chi sigma (tmLam y M)) z then v else E z) (run_substitution_on_tm (cons_substitution y (tmVar (chi sigma (tmLam y M))) sigma) M)) by now apply runLam_ext.
+      intros v.
+      assert (H := IHM (cons_substitution y (tmVar (chi sigma (tmLam y M))) sigma) (fun z : ivar => if ivar_eq_dec (chi sigma (tmLam y M)) z then v else E z)).
+      symmetry in H.
+      symmetry.
+      transitivity (eval_tm (fun z : ivar => eval_tm (fun z0 : ivar => if ivar_eq_dec (chi sigma (tmLam y M)) z0 then v else E z0) (cons_substitution y (tmVar (chi sigma (tmLam y M))) sigma z)) M)...
+      apply eval_tm_ext.
+      intros z H0.
+      unfold cons_substitution.
+      destruct (ivar_eq_dec y z).
+      + unfold eval_tm.
+        destruct (ivar_eq_dec (chi sigma (tmLam y M)) (chi sigma (tmLam y M)))...
+      + apply eval_tm_ext.
+        intros z' H1.
+        destruct (ivar_eq_dec (chi sigma (tmLam y M)) z')...
+        subst.
+        assert (H2 : isFreshIn_substitution (chi sigma (tmLam y M)) sigma (tmLam y M) = true) by now apply main_property_of_chi.
+        unfold isFreshIn_substitution in H2.
+        rewrite forallb_true_iff in H2.
+        enough (H3 : isFreeIn (chi sigma (tmLam y M)) (sigma z) = false) by now rewrite H3 in H1.
+        apply negb_true_iff, H2, getFVs_isFreeIn.
+        simpl.
+        rewrite andb_true_iff, negb_true_iff, Nat.eqb_neq...
+  Qed.
 
-Class isLambdaStructure (Dom : Set) : Type :=
-  { requiresPreLambdaStructure :> isPreLambdaStructure Dom
-  ; respect_beta : forall vv : Dom -> Dom, forall v0 : Dom, runApp (runLam vv) v0 =-= vv v0
-  ; respect_eta : forall v : Dom, runLam (runApp v) =-= v
-  }
-.
+  Class isLambdaStructure (Dom : Type) : Type :=
+    { requiresPreLambdaStructure :> isPreLambdaStructure Dom
+    ; respect_beta : forall vv : Dom -> Dom, forall v0 : Dom, runApp (runLam vv) v0 = vv v0
+    ; respect_eta : forall v : Dom, runLam (runApp v) = v
+    }
+  .
 
-#[global] Hint Resolve respect_beta : semantics_of_ulc.
+  Global Hint Resolve respect_beta : semantics_of_ulc.
 
-#[global] Hint Resolve respect_eta : semantics_of_ulc.
+  Global Hint Resolve respect_eta : semantics_of_ulc.
 
 End UntypedLamdbdaCalculus.
